<?xml version="1.0"?>
<rdf:RDF xmlns="http://www.univ-tours.fr/ipato#"
     xml:base="http://www.univ-tours.fr/ipato"
     xmlns:dc="http://purl.org/dc/elements/1.1/"
     xmlns:owl="http://www.w3.org/2002/07/owl#"
     xmlns:rdf="http://www.w3.org/1999/02/22-rdf-syntax-ns#"
     xmlns:xml="http://www.w3.org/XML/1998/namespace"
     xmlns:xsd="http://www.w3.org/2001/XMLSchema#"
     xmlns:core="http://purl.org/vocab/frbr/core#"
     xmlns:foaf="http://xmlns.com/foaf/0.1/"
     xmlns:obda="https://w3id.org/obda/vocabulary#"
     xmlns:rdfs="http://www.w3.org/2000/01/rdf-schema#"
     xmlns:skos="http://www.w3.org/2004/02/skos/core#"
     xmlns:terms="http://purl.org/dc/terms/"
     xmlns:CRMsci="http://www.ics.forth.gr/isl/CRMsci/"
     xmlns:current="http://erlangen-crm.org/current/light"
     xmlns:bibframe="http://id.loc.gov/ontologies/bibframe/">
    <owl:Ontology rdf:about="http://www.univ-tours.fr/ipato">
        <owl:imports rdf:resource="http://erlangen-crm.org/current/light"/>
        <terms:contributor xml:lang="en">Perrine Thuringer
Damien Vurpillot
Johann Forte
at ARD Intelligence des Patrimoines program, CESR University of Tours, France</terms:contributor>
        <terms:creator xml:lang="en">Developed by:
Emilio M. Sanfilippo
Le Studium Loire Valley Institute for Advanced Studies, and
ARD Intelligence des Patrimoines program, CESR University of Tours, France</terms:creator>
        <rdfs:comment xml:lang="en">This ontology is developed at the ARD Intelligence des Patrimoines program at the CESR University of Tours. The ontology is built on the Erlangen release of CIDOC-CRM v.6.2 but it also covers modeling elements for specific application purposes. These are either taken from existing resources (e.g., Dublin Core, FOAF, DBpedia, etc.) or are newly created.</rdfs:comment>
        <owl:versionInfo xml:lang="en">Status: unstable, work in progress</owl:versionInfo>
    </owl:Ontology>



    <!--
    ///////////////////////////////////////////////////////////////////////////////////////
    //
    // Annotation properties
    //
    ///////////////////////////////////////////////////////////////////////////////////////
     -->




    <!-- http://www.univ-tours.fr/ipato#taxRef_identifier -->

    <owl:AnnotationProperty rdf:about="http://www.univ-tours.fr/ipato#taxRef_identifier"/>



    <!-- http://www.w3.org/2004/02/skos/core#altLabel -->

    <owl:AnnotationProperty rdf:about="http://www.w3.org/2004/02/skos/core#altLabel"/>



    <!-- http://www.w3.org/2004/02/skos/core#definition -->

    <owl:AnnotationProperty rdf:about="http://www.w3.org/2004/02/skos/core#definition"/>



    <!-- http://www.w3.org/2004/02/skos/core#prefLabel -->

    <owl:AnnotationProperty rdf:about="http://www.w3.org/2004/02/skos/core#prefLabel"/>



    <!--
    ///////////////////////////////////////////////////////////////////////////////////////
    //
    // Datatypes
    //
    ///////////////////////////////////////////////////////////////////////////////////////
     -->




    <!-- http://www.w3.org/2001/XMLSchema#date -->

    <rdfs:Datatype rdf:about="http://www.w3.org/2001/XMLSchema#date"/>



    <!-- http://www.w3.org/2001/XMLSchema#gYearMonth -->

    <rdfs:Datatype rdf:about="http://www.w3.org/2001/XMLSchema#gYearMonth"/>



    <!--
    ///////////////////////////////////////////////////////////////////////////////////////
    //
    // Object Properties
    //
    ///////////////////////////////////////////////////////////////////////////////////////
     -->




    <!-- http://dbpedia.org/ontology/birthPlace -->

    <owl:ObjectProperty rdf:about="http://dbpedia.org/ontology/birthPlace">
        <rdfs:domain rdf:resource="http://erlangen-crm.org/current/E21_Person"/>
        <rdfs:range rdf:resource="http://erlangen-crm.org/current/E53_Place"/>
        <rdfs:isDefinedBy rdf:datatype="http://www.w3.org/2001/XMLSchema#anyURI">http://dbpedia.org/ontology/</rdfs:isDefinedBy>
        <skos:prefLabel xml:lang="en">birth place</skos:prefLabel>
    </owl:ObjectProperty>



    <!-- http://dbpedia.org/ontology/deathPlace -->

    <owl:ObjectProperty rdf:about="http://dbpedia.org/ontology/deathPlace">
        <rdfs:domain rdf:resource="http://erlangen-crm.org/current/E21_Person"/>
        <rdfs:range rdf:resource="http://erlangen-crm.org/current/E53_Place"/>
        <rdfs:isDefinedBy rdf:datatype="http://www.w3.org/2001/XMLSchema#anyURI">http://dbpedia.org/ontology/</rdfs:isDefinedBy>
        <skos:prefLabel xml:lang="en">death place</skos:prefLabel>
    </owl:ObjectProperty>



    <!-- http://purl.org/cerif/frapo/hasFundingAgency -->

    <owl:ObjectProperty rdf:about="http://purl.org/cerif/frapo/hasFundingAgency">
        <owl:inverseOf rdf:resource="http://purl.org/cerif/frapo/isFundingAgencyFor"/>
        <rdfs:domain rdf:resource="http://xmlns.com/foaf/0.1/Project"/>
        <rdfs:range rdf:resource="http://www.univ-tours.fr/ipato#FundingAgency"/>
        <rdfs:comment rdf:datatype="http://www.w3.org/2001/XMLSchema#string">In the specific case of the IPATO, hasFundingAgency relates a project to the corresponding funding agency</rdfs:comment>
        <rdfs:isDefinedBy rdf:datatype="http://www.w3.org/2001/XMLSchema#anyURI">https://sparontologies.github.io/frapo/current/frapo.html</rdfs:isDefinedBy>
        <skos:definition rdf:datatype="http://www.w3.org/2001/XMLSchema#string">An object property linking something to a funding agency that provides funding for it</skos:definition>
    </owl:ObjectProperty>



    <!-- http://purl.org/cerif/frapo/isEmployedBy -->

    <owl:ObjectProperty rdf:about="http://purl.org/cerif/frapo/isEmployedBy">
        <rdfs:domain rdf:resource="http://erlangen-crm.org/current/E21_Person"/>
        <rdfs:range>
            <owl:Class>
                <owl:unionOf rdf:parseType="Collection">
                    <rdf:Description rdf:about="http://erlangen-crm.org/current/E40_Legal_Body"/>
                    <rdf:Description rdf:about="http://xmlns.com/foaf/0.1/Organization"/>
                </owl:unionOf>
            </owl:Class>
        </rdfs:range>
        <rdfs:isDefinedBy rdf:datatype="http://www.w3.org/2001/XMLSchema#anyURI">https://sparontologies.github.io/frapo/current/frapo.html</rdfs:isDefinedBy>
    </owl:ObjectProperty>



    <!-- http://purl.org/cerif/frapo/isFundingAgencyFor -->

    <owl:ObjectProperty rdf:about="http://purl.org/cerif/frapo/isFundingAgencyFor">
        <rdfs:domain rdf:resource="http://www.univ-tours.fr/ipato#FundingAgency"/>
        <rdfs:range rdf:resource="http://xmlns.com/foaf/0.1/Project"/>
        <rdfs:comment rdf:datatype="http://www.w3.org/2001/XMLSchema#string">In the specific case of the IPATO, hasFundingAgency relates a project to the corresponding funding agency</rdfs:comment>
        <rdfs:isDefinedBy rdf:datatype="http://www.w3.org/2001/XMLSchema#anyURI">https://sparontologies.github.io/frapo/current/frapo.html</rdfs:isDefinedBy>
        <skos:definition rdf:datatype="http://www.w3.org/2001/XMLSchema#string">An object property linking a funding agency to an entity for which it provides funding</skos:definition>
    </owl:ObjectProperty>



    <!-- http://purl.org/dc/terms/language -->

    <owl:ObjectProperty rdf:about="http://purl.org/dc/terms/language">
        <rdfs:range rdf:resource="http://erlangen-crm.org/current/E56_Language"/>
        <rdfs:comment xml:lang="en">It is not equivalent to CIDOC&apos;s relation E72_has_relation, which relates a linguistic object (e.g., a book&apos;s text) to a language</rdfs:comment>
        <rdfs:isDefinedBy rdf:datatype="http://www.w3.org/2001/XMLSchema#anyURI">https://www.dublincore.org/specifications/dublin-core/dcmi-terms/</rdfs:isDefinedBy>
        <rdfs:label xml:lang="en">language</rdfs:label>
        <skos:definition xml:lang="en">This relation is used to link an entity, e.g., a catalog, to its corresponding (natural) language</skos:definition>
        <skos:prefLabel xml:lang="en">language</skos:prefLabel>
    </owl:ObjectProperty>



    <!-- http://purl.org/dc/terms/subject -->

    <owl:ObjectProperty rdf:about="http://purl.org/dc/terms/subject">
        <rdfs:isDefinedBy rdf:datatype="http://www.w3.org/2001/XMLSchema#anyURI">http://purl.org/dc/terms</rdfs:isDefinedBy>
    </owl:ObjectProperty>



    <!-- http://www.ics.forth.gr/isl/CRMsci/O8_observed -->

    <owl:ObjectProperty rdf:about="http://www.ics.forth.gr/isl/CRMsci/O8_observed">
        <owl:inverseOf rdf:resource="http://www.ics.forth.gr/isl/CRMsci/O8i_was_observed_by"/>
        <rdfs:domain rdf:resource="http://www.ics.forth.gr/isl/CRMsci/S4_Observation"/>
        <rdfs:range rdf:resource="http://erlangen-crm.org/current/E1_CRM_Entity"/>
        <rdfs:isDefinedBy xml:lang="en">http://www.cidoc-crm.org/crmsci/home-1</rdfs:isDefinedBy>
        <skos:prefLabel xml:lang="en">observed</skos:prefLabel>
    </owl:ObjectProperty>



    <!-- http://www.ics.forth.gr/isl/CRMsci/O8i_was_observed_by -->

    <owl:ObjectProperty rdf:about="http://www.ics.forth.gr/isl/CRMsci/O8i_was_observed_by">
        <rdfs:domain rdf:resource="http://erlangen-crm.org/current/E1_CRM_Entity"/>
        <rdfs:range rdf:resource="http://www.ics.forth.gr/isl/CRMsci/S4_Observation"/>
        <rdfs:isDefinedBy xml:lang="en">http://www.cidoc-crm.org/crmsci/home-1</rdfs:isDefinedBy>
        <skos:prefLabel xml:lang="en">was observed by</skos:prefLabel>
    </owl:ObjectProperty>



    <!-- http://www.univ-tours.fr/ipato#archieved_in -->

    <owl:ObjectProperty rdf:about="http://www.univ-tours.fr/ipato#archieved_in">
        <rdfs:domain>
            <owl:Class>
                <owl:unionOf rdf:parseType="Collection">
                    <rdf:Description rdf:about="http://erlangen-crm.org/current/E31_Document"/>
                    <rdf:Description rdf:about="http://erlangen-crm.org/current/E84_Information_Carrier"/>
                    <rdf:Description rdf:about="http://purl.org/vocab/frbr/core#Expression"/>
                </owl:unionOf>
            </owl:Class>
        </rdfs:domain>
        <rdfs:range rdf:resource="http://erlangen-crm.org/current/E53_Place"/>
        <skos:prefLabel xml:lang="en">archieved in</skos:prefLabel>
    </owl:ObjectProperty>



    <!-- http://www.univ-tours.fr/ipato#catalog_of -->

    <owl:ObjectProperty rdf:about="http://www.univ-tours.fr/ipato#catalog_of">
        <owl:inverseOf rdf:resource="http://www.univ-tours.fr/ipato#has_catalog"/>
        <rdfs:label rdf:datatype="http://www.w3.org/2001/XMLSchema#string">catalog of</rdfs:label>
        <skos:prefLabel xml:lang="en">catalog of</skos:prefLabel>
    </owl:ObjectProperty>



    <!-- http://www.univ-tours.fr/ipato#coordinates -->

    <owl:ObjectProperty rdf:about="http://www.univ-tours.fr/ipato#coordinates">
        <owl:inverseOf rdf:resource="http://www.univ-tours.fr/ipato#is_coordinated_by"/>
    </owl:ObjectProperty>



    <!-- http://www.univ-tours.fr/ipato#created_by -->

    <owl:ObjectProperty rdf:about="http://www.univ-tours.fr/ipato#created_by">
        <rdfs:range rdf:resource="http://erlangen-crm.org/current/E39_Actor"/>
        <skos:prefLabel xml:lang="en">created by</skos:prefLabel>
    </owl:ObjectProperty>



    <!-- http://www.univ-tours.fr/ipato#created_in -->

    <owl:ObjectProperty rdf:about="http://www.univ-tours.fr/ipato#created_in">
        <rdfs:domain>
            <owl:Class>
                <owl:unionOf rdf:parseType="Collection">
                    <rdf:Description rdf:about="http://erlangen-crm.org/current/E31_Document"/>
                    <rdf:Description rdf:about="http://erlangen-crm.org/current/E84_Information_Carrier"/>
                    <rdf:Description rdf:about="http://purl.org/vocab/frbr/core#Expression"/>
                </owl:unionOf>
            </owl:Class>
        </rdfs:domain>
        <rdfs:range rdf:resource="http://erlangen-crm.org/current/E53_Place"/>
        <skos:prefLabel xml:lang="en">created in</skos:prefLabel>
    </owl:ObjectProperty>



    <!-- http://www.univ-tours.fr/ipato#edited -->

    <owl:ObjectProperty rdf:about="http://www.univ-tours.fr/ipato#edited">
        <owl:inverseOf rdf:resource="http://www.univ-tours.fr/ipato#edited_by"/>
    </owl:ObjectProperty>



    <!-- http://www.univ-tours.fr/ipato#edited_by -->

    <owl:ObjectProperty rdf:about="http://www.univ-tours.fr/ipato#edited_by">
        <rdfs:domain>
            <owl:Class>
                <owl:unionOf rdf:parseType="Collection">
                    <rdf:Description rdf:about="http://erlangen-crm.org/current/E31_Document"/>
                    <rdf:Description rdf:about="http://erlangen-crm.org/current/E84_Information_Carrier"/>
                    <rdf:Description rdf:about="http://purl.org/vocab/frbr/core#Expression"/>
                </owl:unionOf>
            </owl:Class>
        </rdfs:domain>
        <rdfs:range rdf:resource="http://erlangen-crm.org/current/E21_Person"/>
        <skos:prefLabel xml:lang="en">edited by</skos:prefLabel>
        <skos:prefLabel xml:lang="en">edits</skos:prefLabel>
    </owl:ObjectProperty>



    <!-- http://www.univ-tours.fr/ipato#has_act_form -->

    <owl:ObjectProperty rdf:about="http://www.univ-tours.fr/ipato#has_act_form">
        <rdfs:domain>
            <owl:Class>
                <owl:unionOf rdf:parseType="Collection">
                    <rdf:Description rdf:about="http://erlangen-crm.org/current/E31_Document"/>
                    <rdf:Description rdf:about="http://erlangen-crm.org/current/E84_Information_Carrier"/>
                    <rdf:Description rdf:about="http://purl.org/vocab/frbr/core#Expression"/>
                </owl:unionOf>
            </owl:Class>
        </rdfs:domain>
        <rdfs:range rdf:resource="http://www.univ-tours.fr/ipato#Forme_De_Acte"/>
        <rdfs:comment>This relation is introduced to match experts&apos; terminology with respect to the RENUMAR project</rdfs:comment>
        <skos:prefLabel xml:lang="en">has act from</skos:prefLabel>
    </owl:ObjectProperty>



    <!-- http://www.univ-tours.fr/ipato#has_catalog -->

    <owl:ObjectProperty rdf:about="http://www.univ-tours.fr/ipato#has_catalog">
        <rdfs:domain rdf:resource="http://xmlns.com/foaf/0.1/Project"/>
        <rdfs:range rdf:resource="http://www.w3.org/ns/dcat#Catalog"/>
        <rdfs:label rdf:datatype="http://www.w3.org/2001/XMLSchema#string">has catalog</rdfs:label>
        <skos:prefLabel xml:lang="en">has catalog</skos:prefLabel>
    </owl:ObjectProperty>



    <!-- http://www.univ-tours.fr/ipato#has_project_participant -->

    <owl:ObjectProperty rdf:about="http://www.univ-tours.fr/ipato#has_project_participant">
        <owl:inverseOf rdf:resource="http://www.univ-tours.fr/ipato#participates_in_project"/>
        <rdfs:domain rdf:resource="http://xmlns.com/foaf/0.1/Project"/>
        <rdfs:range rdf:resource="http://erlangen-crm.org/current/E39_Actor"/>
        <rdfs:comment rdf:datatype="http://www.w3.org/2001/XMLSchema#string">This relation has been introduced to explicitly link projects to their participating actors. We do not assume an ontological committment on projects with respect to CIDOC&apos;s taxonomy, e.g., whether they are events or persistent items. This is the reason why has_project_participant is not directly related to the CIDOC&apos;s relation P11_had_participant (which also assumes that a temporal entity is already over)</rdfs:comment>
    </owl:ObjectProperty>



    <!-- http://www.univ-tours.fr/ipato#has_research_area -->

    <owl:ObjectProperty rdf:about="http://www.univ-tours.fr/ipato#has_research_area">
        <rdfs:domain rdf:resource="http://xmlns.com/foaf/0.1/Project"/>
        <rdfs:range rdf:resource="http://www.univ-tours.fr/ipato#Research_Area"/>
    </owl:ObjectProperty>



    <!-- http://www.univ-tours.fr/ipato#has_role -->

    <owl:ObjectProperty rdf:about="http://www.univ-tours.fr/ipato#has_role">
        <rdfs:domain rdf:resource="http://erlangen-crm.org/current/E21_Person"/>
        <rdfs:range rdf:resource="http://id.loc.gov/ontologies/bibframe/Role"/>
        <skos:prefLabel xml:lang="en">has role</skos:prefLabel>
    </owl:ObjectProperty>



    <!-- http://www.univ-tours.fr/ipato#is_about -->

    <owl:ObjectProperty rdf:about="http://www.univ-tours.fr/ipato#is_about">
        <rdfs:domain>
            <owl:Class>
                <owl:unionOf rdf:parseType="Collection">
                    <rdf:Description rdf:about="http://www.w3.org/ns/dcat#Catalog"/>
                    <rdf:Description rdf:about="http://www.w3.org/ns/dcat#Dataset"/>
                    <rdf:Description rdf:about="http://xmlns.com/foaf/0.1/Project"/>
                </owl:unionOf>
            </owl:Class>
        </rdfs:domain>
        <rdfs:range rdf:resource="http://erlangen-crm.org/current/E1_CRM_Entity"/>
        <rdfs:comment rdf:datatype="http://www.w3.org/2001/XMLSchema#string">CIDOC&apos;s relation P129_is_about has a different intended meaning; for this reason, P129 and is_about are not equivalent</rdfs:comment>
        <skos:definition rdf:datatype="http://www.w3.org/2001/XMLSchema#string">This relation is used to link a resource like a project or a catalog to the entities it is about. For instance, in the context of cultural heritage, a project could be about manuscripts, statues, paintings, etc.</skos:definition>
    </owl:ObjectProperty>



    <!-- http://www.univ-tours.fr/ipato#is_associated_to -->

    <owl:ObjectProperty rdf:about="http://www.univ-tours.fr/ipato#is_associated_to">
        <rdfs:domain rdf:resource="http://xmlns.com/foaf/0.1/Project"/>
        <rdfs:range rdf:resource="http://xmlns.com/foaf/0.1/Group"/>
        <rdfs:comment rdf:datatype="http://www.w3.org/2001/XMLSchema#string">This relation is used to link a project to a group of agents, e.g., the project Renumar is_associated_to a research group at the CESR University of Tours</rdfs:comment>
    </owl:ObjectProperty>



    <!-- http://www.univ-tours.fr/ipato#is_coordinated_by -->

    <owl:ObjectProperty rdf:about="http://www.univ-tours.fr/ipato#is_coordinated_by">
        <rdfs:domain rdf:resource="http://xmlns.com/foaf/0.1/Project"/>
        <rdfs:range rdf:resource="http://xmlns.com/foaf/0.1/Person"/>
    </owl:ObjectProperty>



    <!-- http://www.univ-tours.fr/ipato#is_found_with -->

    <owl:ObjectProperty rdf:about="http://www.univ-tours.fr/ipato#is_found_with">
        <rdfs:domain>
            <owl:Class>
                <owl:unionOf rdf:parseType="Collection">
                    <rdf:Description rdf:about="http://erlangen-crm.org/current/E27_Site"/>
                    <rdf:Description rdf:about="http://erlangen-crm.org/current/E53_Place"/>
                </owl:unionOf>
            </owl:Class>
        </rdfs:domain>
        <skos:prefLabel xml:lang="en">is found with</skos:prefLabel>
    </owl:ObjectProperty>



    <!-- http://www.univ-tours.fr/ipato#participates_in_project -->

    <owl:ObjectProperty rdf:about="http://www.univ-tours.fr/ipato#participates_in_project"/>



    <!-- http://www.w3.org/ns/dcat#dataset -->

    <owl:ObjectProperty rdf:about="http://www.w3.org/ns/dcat#dataset">
        <rdfs:domain rdf:resource="http://www.w3.org/ns/dcat#Catalog"/>
        <rdfs:range rdf:resource="http://www.w3.org/ns/dcat#Dataset"/>
        <rdfs:comment rdf:datatype="http://www.w3.org/2001/XMLSchema#string">A collection of data that is listed in the catalog</rdfs:comment>
        <rdfs:isDefinedBy rdf:datatype="http://www.w3.org/2001/XMLSchema#anyURI">https://www.w3.org/TR/vocab-dcat-2/</rdfs:isDefinedBy>
        <rdfs:isDefinedBy rdf:datatype="http://www.w3.org/2001/XMLSchema#anyURI">https://www.w3.org/ns/dcat.html</rdfs:isDefinedBy>
    </owl:ObjectProperty>



    <!--
    ///////////////////////////////////////////////////////////////////////////////////////
    //
    // Data properties
    //
    ///////////////////////////////////////////////////////////////////////////////////////
     -->




    <!-- http://dbpedia.org/ontology/birthDate -->

    <owl:DatatypeProperty rdf:about="http://dbpedia.org/ontology/birthDate">
        <rdfs:domain rdf:resource="http://erlangen-crm.org/current/E21_Person"/>
        <rdfs:range rdf:resource="http://www.w3.org/2000/01/rdf-schema#Literal"/>
        <rdfs:isDefinedBy rdf:datatype="http://www.w3.org/2001/XMLSchema#anyURI">http://dbpedia.org/ontology/</rdfs:isDefinedBy>
    </owl:DatatypeProperty>



    <!-- http://dbpedia.org/ontology/deathDate -->

    <owl:DatatypeProperty rdf:about="http://dbpedia.org/ontology/deathDate">
        <rdfs:domain rdf:resource="http://erlangen-crm.org/current/E21_Person"/>
        <rdfs:range rdf:resource="http://www.w3.org/2000/01/rdf-schema#Literal"/>
        <rdfs:isDefinedBy rdf:datatype="http://www.w3.org/2001/XMLSchema#anyURI">http://dbpedia.org/ontology/</rdfs:isDefinedBy>
    </owl:DatatypeProperty>



    <!-- http://id.loc.gov/ontologies/bibframe/ShelfMark -->

    <owl:DatatypeProperty rdf:about="http://id.loc.gov/ontologies/bibframe/ShelfMark">
        <rdfs:range rdf:resource="http://www.w3.org/2000/01/rdf-schema#Literal"/>
        <rdfs:comment>Imported from BibFrame.
http://id.loc.gov/ontologies/bibframe.html#</rdfs:comment>
        <skos:prefLabel xml:lang="en">shelfmark</skos:prefLabel>
    </owl:DatatypeProperty>



    <!-- http://purl.org/dc/terms/created -->

    <owl:DatatypeProperty rdf:about="http://purl.org/dc/terms/created">
        <rdfs:range rdf:resource="http://www.w3.org/2000/01/rdf-schema#Literal"/>
        <rdfs:isDefinedBy rdf:datatype="http://www.w3.org/2001/XMLSchema#anyURI">http://purl.org/dc/terms</rdfs:isDefinedBy>
    </owl:DatatypeProperty>



    <!-- http://purl.org/dc/terms/date -->

    <owl:DatatypeProperty rdf:about="http://purl.org/dc/terms/date">
        <rdfs:domain rdf:resource="http://erlangen-crm.org/current/E1_CRM_Entity"/>
        <rdfs:range rdf:resource="http://www.w3.org/2000/01/rdf-schema#Literal"/>
        <rdfs:isDefinedBy rdf:datatype="http://www.w3.org/2001/XMLSchema#anyURI">http://purl.org/dc/terms</rdfs:isDefinedBy>
    </owl:DatatypeProperty>



    <!-- http://purl.org/dc/terms/description -->

    <owl:DatatypeProperty rdf:about="http://purl.org/dc/terms/description">
        <rdfs:range rdf:resource="http://www.w3.org/2001/XMLSchema#string"/>
        <rdfs:isDefinedBy rdf:datatype="http://www.w3.org/2001/XMLSchema#anyURI">http://purl.org/dc/terms</rdfs:isDefinedBy>
    </owl:DatatypeProperty>



    <!-- http://purl.org/dc/terms/format -->

    <owl:DatatypeProperty rdf:about="http://purl.org/dc/terms/format">
        <rdfs:range rdf:resource="http://www.w3.org/2001/XMLSchema#string"/>
        <rdfs:isDefinedBy rdf:datatype="http://www.w3.org/2001/XMLSchema#anyURI">https://www.dublincore.org/specifications/dublin-core/dcmi-terms/</rdfs:isDefinedBy>
    </owl:DatatypeProperty>



    <!-- http://purl.org/dc/terms/identifier -->

    <owl:DatatypeProperty rdf:about="http://purl.org/dc/terms/identifier"/>



    <!-- http://purl.org/dc/terms/publisher -->

    <owl:DatatypeProperty rdf:about="http://purl.org/dc/terms/publisher">
        <rdfs:isDefinedBy rdf:datatype="http://www.w3.org/2001/XMLSchema#anyURI">https://www.dublincore.org/specifications/dublin-core/dcmi-terms/</rdfs:isDefinedBy>
    </owl:DatatypeProperty>



    <!-- http://purl.org/dc/terms/rights -->

    <owl:DatatypeProperty rdf:about="http://purl.org/dc/terms/rights">
        <rdfs:range rdf:resource="http://www.w3.org/2001/XMLSchema#string"/>
        <rdfs:isDefinedBy rdf:datatype="http://www.w3.org/2001/XMLSchema#anyURI">https://www.dublincore.org/specifications/dublin-core/dcmi-terms/</rdfs:isDefinedBy>
    </owl:DatatypeProperty>



    <!-- http://purl.org/dc/terms/title -->

    <owl:DatatypeProperty rdf:about="http://purl.org/dc/terms/title">
        <rdfs:range rdf:resource="http://www.w3.org/2001/XMLSchema#string"/>
    </owl:DatatypeProperty>



    <!-- http://schema.org/email -->

    <owl:DatatypeProperty rdf:about="http://schema.org/email">
        <rdfs:range rdf:resource="http://www.w3.org/2001/XMLSchema#anyURI"/>
        <rdfs:isDefinedBy rdf:datatype="http://www.w3.org/2001/XMLSchema#anyURI">https://schema.org/</rdfs:isDefinedBy>
    </owl:DatatypeProperty>



    <!-- http://schema.org/url -->

    <owl:DatatypeProperty rdf:about="http://schema.org/url">
        <rdfs:range rdf:resource="http://www.w3.org/2001/XMLSchema#anyURI"/>
        <rdfs:isDefinedBy rdf:datatype="http://www.w3.org/2001/XMLSchema#anyURI">https://schema.org</rdfs:isDefinedBy>
    </owl:DatatypeProperty>



    <!-- http://www.univ-tours.fr/ipato#dataCite_identifier -->

    <owl:DatatypeProperty rdf:about="http://www.univ-tours.fr/ipato#dataCite_identifier">
        <rdfs:domain rdf:resource="http://www.w3.org/ns/dcat#Dataset"/>
        <rdfs:range rdf:resource="http://www.w3.org/2000/01/rdf-schema#Literal"/>
    </owl:DatatypeProperty>



    <!-- http://www.univ-tours.fr/ipato#dataIPAT_identifier -->

    <owl:DatatypeProperty rdf:about="http://www.univ-tours.fr/ipato#dataIPAT_identifier">
        <rdfs:domain rdf:resource="http://www.w3.org/ns/dcat#Dataset"/>
        <rdfs:range rdf:resource="http://www.w3.org/2000/01/rdf-schema#Literal"/>
    </owl:DatatypeProperty>



    <!-- http://www.univ-tours.fr/ipato#renumar_identifier -->

    <owl:DatatypeProperty rdf:about="http://www.univ-tours.fr/ipato#renumar_identifier">
        <rdfs:range rdf:resource="http://www.w3.org/2000/01/rdf-schema#Literal"/>
        <skos:prefLabel xml:lang="en">renumar identifier</skos:prefLabel>
    </owl:DatatypeProperty>



    <!-- http://www.w3.org/ns/dcat#accessURL -->

    <owl:DatatypeProperty rdf:about="http://www.w3.org/ns/dcat#accessURL">
        <rdfs:range rdf:resource="http://www.w3.org/2001/XMLSchema#anyURI"/>
        <rdfs:isDefinedBy rdf:datatype="http://www.w3.org/2001/XMLSchema#anyURI">https://www.w3.org/TR/vocab-dcat-2/</rdfs:isDefinedBy>
    </owl:DatatypeProperty>



    <!-- http://xmlns.com/foaf/0.1/firstName -->

    <owl:DatatypeProperty rdf:about="http://xmlns.com/foaf/0.1/firstName">
        <rdfs:domain rdf:resource="http://erlangen-crm.org/current/E21_Person"/>
        <rdfs:range rdf:resource="http://www.w3.org/2001/XMLSchema#string"/>
        <rdfs:isDefinedBy rdf:datatype="http://www.w3.org/2001/XMLSchema#anyURI">http://xmlns.com/foaf/spec/</rdfs:isDefinedBy>
    </owl:DatatypeProperty>



    <!-- http://xmlns.com/foaf/0.1/lastName -->

    <owl:DatatypeProperty rdf:about="http://xmlns.com/foaf/0.1/lastName">
        <rdfs:domain rdf:resource="http://erlangen-crm.org/current/E21_Person"/>
        <rdfs:range rdf:resource="http://www.w3.org/2001/XMLSchema#string"/>
        <rdfs:isDefinedBy rdf:datatype="http://www.w3.org/2001/XMLSchema#anyURI">http://xmlns.com/foaf/spec/</rdfs:isDefinedBy>
    </owl:DatatypeProperty>



    <!-- http://xmlns.com/foaf/0.1/mbox -->

    <owl:DatatypeProperty rdf:about="http://xmlns.com/foaf/0.1/mbox">
        <rdfs:domain rdf:resource="http://erlangen-crm.org/current/E39_Actor"/>
        <rdfs:range rdf:resource="http://www.w3.org/2001/XMLSchema#anyURI"/>
    </owl:DatatypeProperty>



    <!-- http://xmlns.com/foaf/0.1/name -->

    <owl:DatatypeProperty rdf:about="http://xmlns.com/foaf/0.1/name">
        <rdfs:domain rdf:resource="http://erlangen-crm.org/current/E39_Actor"/>
        <rdfs:range rdf:resource="http://www.w3.org/2001/XMLSchema#string"/>
        <rdfs:isDefinedBy rdf:datatype="http://www.w3.org/2001/XMLSchema#anyURI">http://xmlns.com/foaf/spec/</rdfs:isDefinedBy>
    </owl:DatatypeProperty>



    <!-- https://w3id.org/arco/ontology/arco/endTime -->

    <owl:DatatypeProperty rdf:about="https://w3id.org/arco/ontology/arco/endTime">
        <rdfs:range rdf:resource="http://www.w3.org/2000/01/rdf-schema#Literal"/>
        <rdfs:isDefinedBy rdf:datatype="http://www.w3.org/2001/XMLSchema#anyURI">http://wit.istc.cnr.it/arco</rdfs:isDefinedBy>
    </owl:DatatypeProperty>



    <!-- https://w3id.org/arco/ontology/arco/startTime -->

    <owl:DatatypeProperty rdf:about="https://w3id.org/arco/ontology/arco/startTime">
        <rdfs:range rdf:resource="http://www.w3.org/2000/01/rdf-schema#Literal"/>
        <rdfs:isDefinedBy rdf:datatype="http://www.w3.org/2001/XMLSchema#anyURI">http://wit.istc.cnr.it/arco</rdfs:isDefinedBy>
    </owl:DatatypeProperty>



    <!-- https://www.geonames.org/ontology#lat -->

    <owl:DatatypeProperty rdf:about="https://www.geonames.org/ontology#lat">
        <rdfs:domain>
            <owl:Class>
                <owl:unionOf rdf:parseType="Collection">
                    <rdf:Description rdf:about="http://erlangen-crm.org/current/E27_Site"/>
                    <rdf:Description rdf:about="http://erlangen-crm.org/current/E53_Place"/>
                </owl:unionOf>
            </owl:Class>
        </rdfs:domain>
        <rdfs:range>
            <rdfs:Datatype>
                <owl:unionOf rdf:parseType="Collection">
                    <rdf:Description rdf:about="http://www.w3.org/2000/01/rdf-schema#Literal"/>
                    <rdf:Description rdf:about="http://www.w3.org/2001/XMLSchema#decimal"/>
                </owl:unionOf>
            </rdfs:Datatype>
        </rdfs:range>
        <rdfs:comment rdf:datatype="http://www.w3.org/2001/XMLSchema#string">latitude of a resource (decimal degrees)</rdfs:comment>
        <rdfs:isDefinedBy rdf:datatype="http://www.w3.org/2001/XMLSchema#anyURI">http://www.geonames.org/ontology/ontology_v3.2.rdf</rdfs:isDefinedBy>
        <rdfs:label rdf:datatype="http://www.w3.org/2001/XMLSchema#string">latitude</rdfs:label>
        <skos:prefLabel xml:lang="en">latitude</skos:prefLabel>
    </owl:DatatypeProperty>



    <!-- https://www.geonames.org/ontology#long -->

    <owl:DatatypeProperty rdf:about="https://www.geonames.org/ontology#long">
        <rdfs:domain>
            <owl:Class>
                <owl:unionOf rdf:parseType="Collection">
                    <rdf:Description rdf:about="http://erlangen-crm.org/current/E27_Site"/>
                    <rdf:Description rdf:about="http://erlangen-crm.org/current/E53_Place"/>
                </owl:unionOf>
            </owl:Class>
        </rdfs:domain>
        <rdfs:range rdf:resource="http://www.w3.org/2000/01/rdf-schema#Literal"/>
        <rdfs:comment xml:lang="en">longitude of a resource (decimal degrees)</rdfs:comment>
        <rdfs:isDefinedBy rdf:datatype="http://www.w3.org/2001/XMLSchema#anyURI">http://www.geonames.org/ontology/ontology_v3.2.rdf</rdfs:isDefinedBy>
        <rdfs:label rdf:datatype="http://www.w3.org/2001/XMLSchema#string">longitude</rdfs:label>
        <skos:prefLabel xml:lang="en">longitude</skos:prefLabel>
    </owl:DatatypeProperty>



    <!-- https://www.geonames.org/ontology#population -->

    <owl:DatatypeProperty rdf:about="https://www.geonames.org/ontology#population">
        <rdfs:isDefinedBy rdf:datatype="http://www.w3.org/2001/XMLSchema#anyURI">http://www.geonames.org/ontology/ontology_v3.2.rdf</rdfs:isDefinedBy>
        <rdfs:label rdf:datatype="http://www.w3.org/2001/XMLSchema#string">population</rdfs:label>
        <skos:prefLabel xml:lang="en">population</skos:prefLabel>
    </owl:DatatypeProperty>



    <!-- https://www.geonames.org/ontology#postalCode -->

    <owl:DatatypeProperty rdf:about="https://www.geonames.org/ontology#postalCode">
        <rdfs:isDefinedBy rdf:datatype="http://www.w3.org/2001/XMLSchema#anyURI">http://www.geonames.org/ontology/ontology_v3.2.rdf</rdfs:isDefinedBy>
        <rdfs:label rdf:datatype="http://www.w3.org/2001/XMLSchema#string">postal code</rdfs:label>
        <skos:prefLabel xml:lang="en">postal code</skos:prefLabel>
    </owl:DatatypeProperty>



    <!--
    ///////////////////////////////////////////////////////////////////////////////////////
    //
    // Classes
    //
    ///////////////////////////////////////////////////////////////////////////////////////
     -->




    <!-- http://dbpedia.org/ontology/City -->

    <owl:Class rdf:about="http://dbpedia.org/ontology/City">
        <rdfs:subClassOf rdf:resource="http://dbpedia.org/ontology/PopulatedPlace"/>
        <owl:disjointWith rdf:resource="http://dbpedia.org/ontology/Country"/>
        <owl:disjointWith rdf:resource="http://dbpedia.org/ontology/Library"/>
        <owl:disjointWith rdf:resource="http://www.univ-tours.fr/ipato#French_Department"/>
        <owl:disjointWith rdf:resource="http://www.univ-tours.fr/ipato#French_Region"/>
        <rdfs:isDefinedBy rdf:datatype="http://www.w3.org/2001/XMLSchema#anyURI">https://wiki.dbpedia.org/services-resources/ontology</rdfs:isDefinedBy>
        <rdfs:label rdf:datatype="http://www.w3.org/2001/XMLSchema#string">City</rdfs:label>
        <skos:definition rdf:datatype="http://www.w3.org/2001/XMLSchema#string">A city is a large and permanent human settlement. Although there is no agreement on how a city is distinguished from a town in general English language meanings, many cities have a particular administrative, legal, or historical status based on local law. Cities generally have complex systems for sanitation, utilities, land usage, housing, and transportation. The concentration of development greatly facilitates interaction between people and businesses, sometimes benefiting both parties in the process, but it also presents challenges to managing urban growth.</skos:definition>
        <skos:prefLabel xml:lang="en">City</skos:prefLabel>
        <skos:prefLabel xml:lang="fr">Ville</skos:prefLabel>
    </owl:Class>



    <!-- http://dbpedia.org/ontology/Country -->

    <owl:Class rdf:about="http://dbpedia.org/ontology/Country">
        <rdfs:subClassOf rdf:resource="http://dbpedia.org/ontology/PopulatedPlace"/>
        <owl:disjointWith rdf:resource="http://dbpedia.org/ontology/Library"/>
        <owl:disjointWith rdf:resource="http://www.univ-tours.fr/ipato#French_Department"/>
        <owl:disjointWith rdf:resource="http://www.univ-tours.fr/ipato#French_Region"/>
        <rdfs:isDefinedBy rdf:datatype="http://www.w3.org/2001/XMLSchema#anyURI">https://wiki.dbpedia.org/services-resources/ontology</rdfs:isDefinedBy>
        <rdfs:label xml:lang="en">Country</rdfs:label>
        <skos:prefLabel xml:lang="en">Country</skos:prefLabel>
        <skos:prefLabel xml:lang="fr">Pays</skos:prefLabel>
    </owl:Class>



    <!-- http://dbpedia.org/ontology/Library -->

    <owl:Class rdf:about="http://dbpedia.org/ontology/Library">
        <rdfs:subClassOf rdf:resource="http://erlangen-crm.org/current/E53_Place"/>
        <owl:disjointWith rdf:resource="http://www.univ-tours.fr/ipato#French_Department"/>
        <owl:disjointWith rdf:resource="http://www.univ-tours.fr/ipato#French_Region"/>
        <rdfs:isDefinedBy rdf:datatype="http://www.w3.org/2001/XMLSchema#anyURI">http://dbpedia.org/ontology/</rdfs:isDefinedBy>
        <rdfs:label xml:lang="en">Library</rdfs:label>
        <skos:prefLabel xml:lang="en">Library</skos:prefLabel>
        <skos:prefLabel xml:lang="fr">bibliothèque</skos:prefLabel>
    </owl:Class>



    <!-- http://dbpedia.org/ontology/PopulatedPlace -->

    <owl:Class rdf:about="http://dbpedia.org/ontology/PopulatedPlace">
        <rdfs:subClassOf rdf:resource="http://erlangen-crm.org/current/E53_Place"/>
        <rdfs:isDefinedBy rdf:datatype="http://www.w3.org/2001/XMLSchema#anyURI">https://wiki.dbpedia.org/services-resources/ontology</rdfs:isDefinedBy>
        <rdfs:label rdf:datatype="http://www.w3.org/2001/XMLSchema#string">Populated place</rdfs:label>
        <skos:definition rdf:datatype="http://www.w3.org/2001/XMLSchema#string">As defined by the United States Geological Survey, a populated place is a place or area with clustered or scattered buildings and a permanent human population (city, settlement, town, or village) referenced with geographic coordinates (http://en.wikipedia.org/wiki/Populated_place). (en)</skos:definition>
        <skos:prefLabel xml:lang="en">Populated place</skos:prefLabel>
        <skos:prefLabel xml:lang="fr">lieu habité</skos:prefLabel>
    </owl:Class>



    <!-- http://erlangen-crm.org/current/E1_CRM_Entity -->

    <rdf:Description rdf:about="http://erlangen-crm.org/current/E1_CRM_Entity">
        <rdfs:label xml:lang="en">CRM Entity</rdfs:label>
    </rdf:Description>



    <!-- http://erlangen-crm.org/current/E21_Person -->

    <rdf:Description rdf:about="http://erlangen-crm.org/current/E21_Person">
        <owl:equivalentClass rdf:resource="http://xmlns.com/foaf/0.1/Person"/>
    </rdf:Description>



    <!-- http://erlangen-crm.org/current/E39_Actor -->

    <rdf:Description rdf:about="http://erlangen-crm.org/current/E39_Actor">
        <owl:equivalentClass rdf:resource="http://xmlns.com/foaf/0.1/Agent"/>
        <rdfs:subClassOf>
            <owl:Restriction>
                <owl:onProperty rdf:resource="http://xmlns.com/foaf/0.1/name"/>
                <owl:allValuesFrom rdf:resource="http://www.w3.org/2001/XMLSchema#string"/>
            </owl:Restriction>
        </rdfs:subClassOf>
    </rdf:Description>



    <!-- http://erlangen-crm.org/current/E53_Place -->

    <rdf:Description rdf:about="http://erlangen-crm.org/current/E53_Place">
        <rdfs:subClassOf>
            <owl:Restriction>
                <owl:onProperty rdf:resource="https://www.geonames.org/ontology#lat"/>
                <owl:someValuesFrom rdf:resource="http://www.w3.org/2000/01/rdf-schema#Literal"/>
            </owl:Restriction>
        </rdfs:subClassOf>
        <rdfs:subClassOf>
            <owl:Restriction>
                <owl:onProperty rdf:resource="https://www.geonames.org/ontology#long"/>
                <owl:someValuesFrom rdf:resource="http://www.w3.org/2000/01/rdf-schema#Literal"/>
            </owl:Restriction>
        </rdfs:subClassOf>
    </rdf:Description>



    <!-- http://erlangen-crm.org/current/E70_Thing -->

    <rdf:Description rdf:about="http://erlangen-crm.org/current/E70_Thing">
        <rdfs:subClassOf>
            <owl:Restriction>
                <owl:onProperty rdf:resource="http://erlangen-crm.org/current/P43_has_dimension"/>
                <owl:someValuesFrom rdf:resource="http://erlangen-crm.org/current/E54_Dimension"/>
            </owl:Restriction>
        </rdfs:subClassOf>
    </rdf:Description>



    <!-- http://erlangen-crm.org/current/E71_Man-Made_Thing -->

    <rdf:Description rdf:about="http://erlangen-crm.org/current/E71_Man-Made_Thing">
        <rdfs:subClassOf>
            <owl:Restriction>
                <owl:onProperty rdf:resource="http://www.univ-tours.fr/ipato#created_by"/>
                <owl:someValuesFrom rdf:resource="http://erlangen-crm.org/current/E39_Actor"/>
            </owl:Restriction>
        </rdfs:subClassOf>
    </rdf:Description>



    <!-- http://erlangen-crm.org/current/E74_Group -->

    <rdf:Description rdf:about="http://erlangen-crm.org/current/E74_Group">
        <owl:equivalentClass rdf:resource="http://xmlns.com/foaf/0.1/Group"/>
    </rdf:Description>



    <!-- http://erlangen-crm.org/current/E84_Information_Carrier -->

    <rdf:Description rdf:about="http://erlangen-crm.org/current/E84_Information_Carrier">
        <rdfs:subClassOf>
            <owl:Restriction>
                <owl:onProperty rdf:resource="http://erlangen-crm.org/current/P128_carries"/>
                <owl:someValuesFrom rdf:resource="http://erlangen-crm.org/current/E89_Propositional_Object"/>
            </owl:Restriction>
        </rdfs:subClassOf>
    </rdf:Description>



    <!-- http://id.loc.gov/ontologies/bibframe/Role -->

    <owl:Class rdf:about="http://id.loc.gov/ontologies/bibframe/Role">
        <rdfs:subClassOf rdf:resource="http://erlangen-crm.org/current/E55_Type"/>
    </owl:Class>



    <!-- http://purl.org/vocab/frbr/core#Expression -->

    <owl:Class rdf:about="http://purl.org/vocab/frbr/core#Expression">
        <rdfs:subClassOf rdf:resource="http://erlangen-crm.org/current/E73_Information_Object"/>
        <rdfs:subClassOf>
            <owl:Restriction>
                <owl:onProperty rdf:resource="http://erlangen-crm.org/current/P128i_is_carried_by"/>
                <owl:someValuesFrom rdf:resource="http://erlangen-crm.org/current/E84_Information_Carrier"/>
            </owl:Restriction>
        </rdfs:subClassOf>
        <rdfs:isDefinedBy>Class taken from core structure of FRBR

https://sparontologies.github.io/frbr/current/frbr.html#d4e1431</rdfs:isDefinedBy>
    </owl:Class>



    <!-- http://www.ics.forth.gr/isl/CRMsci/S4_Observation -->

    <owl:Class rdf:about="http://www.ics.forth.gr/isl/CRMsci/S4_Observation">
        <rdfs:subClassOf rdf:resource="http://erlangen-crm.org/current/E13_Attribute_Assignment"/>
        <rdfs:comment>This class comprises the activity of gaining scientific knowledge about particular states of physical reality gained by empirical evidence, experiments and by measurements. We define observation in the sense of natural sciences, as a kind of human activity: at some Place and within some Time-Span, certain Physical Things and their behavior and interactions are observed, either directly by human sensory impression, or enhanced with tools and measurement devices. The output of the internal processes of measurement devices that do not require additional human interaction are in general regarded as part of the observation and not as additional inference. Manual recordings may serve as additional evidence. Measurements and witnessing of events are special cases of observations. Observations result in a belief about certain propositions. In this model, the degree of confidence in the observed properties is regarded to be “true” per default, but could be described differently by adding a property P3 has note to an instance of S4 Observation, or by reification of the property O16 observed value. Primary data from measurement devices are regarded in this model to be results of observation and can be interpreted as propositions believed to be true within the (known) tolerances and degree of reliability of the device. Observations represent the transition between reality and propositions in the form of instances of a formal ontology, and can be subject to data evaluation from this point on.</rdfs:comment>
        <rdfs:isDefinedBy>CRMSci</rdfs:isDefinedBy>
    </owl:Class>



    <!-- http://www.univ-tours.fr/ipato#Acte_privé -->

    <owl:Class rdf:about="http://www.univ-tours.fr/ipato#Acte_privé">
        <rdfs:subClassOf rdf:resource="http://erlangen-crm.org/current/E31_Document"/>
        <rdfs:seeAlso xml:lang="en">https://legal-dictionary.thefreedictionary.com/Private+act</rdfs:seeAlso>
        <skos:altLabel xml:lang="fr">Private act</skos:altLabel>
        <skos:definition xml:lang="en">a statute exclusively for the settlement of private
and personal interests, of which courts do not take
judicial notice; - opposed to a general law, which
operates on the whole community</skos:definition>
        <skos:prefLabel xml:lang="fr">Acte privé</skos:prefLabel>
    </owl:Class>



    <!-- http://www.univ-tours.fr/ipato#Archive -->

    <owl:Class rdf:about="http://www.univ-tours.fr/ipato#Archive">
        <rdfs:subClassOf rdf:resource="http://erlangen-crm.org/current/E53_Place"/>
    </owl:Class>



    <!-- http://www.univ-tours.fr/ipato#Expédition_notariale -->

    <owl:Class rdf:about="http://www.univ-tours.fr/ipato#Expédition_notariale">
        <rdfs:subClassOf rdf:resource="http://erlangen-crm.org/current/E31_Document"/>
        <skos:altLabel xml:lang="fr">Notarial deed</skos:altLabel>
        <skos:definition xml:lang="fr">Acte notarié qui est adressé à un particulier et qui témoigne de l&apos;accord
passé devant le notaire.</skos:definition>
        <skos:prefLabel xml:lang="fr">Expédition notariale</skos:prefLabel>
    </owl:Class>



    <!-- http://www.univ-tours.fr/ipato#Forme_De_Acte -->

    <owl:Class rdf:about="http://www.univ-tours.fr/ipato#Forme_De_Acte">
        <rdfs:subClassOf rdf:resource="http://erlangen-crm.org/current/E55_Type"/>
        <rdfs:subClassOf>
            <owl:Restriction>
                <owl:onProperty rdf:resource="http://erlangen-crm.org/current/P2i_is_type_of"/>
                <owl:someValuesFrom rdf:resource="http://erlangen-crm.org/current/E31_Document"/>
            </owl:Restriction>
        </rdfs:subClassOf>
        <rdfs:subClassOf>
            <owl:Restriction>
                <owl:onProperty rdf:resource="http://erlangen-crm.org/current/P2i_is_type_of"/>
                <owl:allValuesFrom>
                    <owl:Class>
                        <owl:unionOf rdf:parseType="Collection">
                            <rdf:Description rdf:about="http://erlangen-crm.org/current/E31_Document"/>
                            <rdf:Description rdf:about="http://erlangen-crm.org/current/E84_Information_Carrier"/>
                            <rdf:Description rdf:about="http://purl.org/vocab/frbr/core#Expression"/>
                        </owl:unionOf>
                    </owl:Class>
                </owl:allValuesFrom>
            </owl:Restriction>
        </rdfs:subClassOf>
        <rdfs:comment xml:lang="en">This class has been added in the context of the RENUMAR project to represent types of historical documents</rdfs:comment>
        <skos:altLabel xml:lang="en">Subject of Document</skos:altLabel>
        <skos:prefLabel xml:lang="fr">Forme de l&apos;acte</skos:prefLabel>
    </owl:Class>



    <!-- http://www.univ-tours.fr/ipato#French_Department -->

    <owl:Class rdf:about="http://www.univ-tours.fr/ipato#French_Department">
        <rdfs:subClassOf rdf:resource="http://dbpedia.org/ontology/PopulatedPlace"/>
        <owl:disjointWith rdf:resource="http://www.univ-tours.fr/ipato#French_Region"/>
    </owl:Class>



    <!-- http://www.univ-tours.fr/ipato#French_Region -->

    <owl:Class rdf:about="http://www.univ-tours.fr/ipato#French_Region">
        <rdfs:subClassOf rdf:resource="http://dbpedia.org/ontology/PopulatedPlace"/>
    </owl:Class>



    <!-- http://www.univ-tours.fr/ipato#FundingAgency -->

    <owl:Class rdf:about="http://www.univ-tours.fr/ipato#FundingAgency">
        <rdfs:subClassOf rdf:resource="http://xmlns.com/foaf/0.1/Organization"/>
        <rdfs:isDefinedBy rdf:datatype="http://www.w3.org/2001/XMLSchema#anyURI">https://sparontologies.github.io/frapo/current/frapo.html</rdfs:isDefinedBy>
    </owl:Class>



    <!-- http://www.univ-tours.fr/ipato#Lettre -->

    <owl:Class rdf:about="http://www.univ-tours.fr/ipato#Lettre">
        <rdfs:subClassOf rdf:resource="http://erlangen-crm.org/current/E31_Document"/>
        <skos:definition xml:lang="fr">Acte épistolaire de nature privée.</skos:definition>
        <skos:prefLabel xml:lang="fr">Lettre</skos:prefLabel>
    </owl:Class>



    <!-- http://www.univ-tours.fr/ipato#Lettre_close -->

    <owl:Class rdf:about="http://www.univ-tours.fr/ipato#Lettre_close">
        <rdfs:subClassOf rdf:resource="http://erlangen-crm.org/current/E31_Document"/>
        <skos:definition xml:lang="fr">Lettre du roi à une autorité collective comme à un individu, exprimant un ordre, et expédiée fermée du sceau du secret de cire rouge et présentant certains caractères diplomatiques nettement caractérisés (petite dimension, propos courts, précédés de l&apos;expression &quot;De par le roy&quot;, formule de corroboration, ni d&apos;annonce de sceau).</skos:definition>
        <skos:prefLabel xml:lang="fr">Lettre close</skos:prefLabel>
    </owl:Class>



    <!-- http://www.univ-tours.fr/ipato#Lettre_de_cachet -->

    <owl:Class rdf:about="http://www.univ-tours.fr/ipato#Lettre_de_cachet">
        <rdfs:subClassOf rdf:resource="http://erlangen-crm.org/current/E31_Document"/>
        <skos:altLabel xml:lang="fr">lettre close</skos:altLabel>
        <skos:altLabel xml:lang="fr">lettre fermée</skos:altLabel>
        <skos:definition xml:lang="fr">Une lettre de cachet  est, sous l’Ancien Régime
en France, une lettre servant à la
transmission d’un ordre particulier du roi,
permettant par exemple l&apos;incarcération sans jugement,
l&apos;exil ou encore l&apos;internement de personnes jugées
indésirables par le pouvoir.</skos:definition>
        <skos:prefLabel xml:lang="fr">Lettre de cachet</skos:prefLabel>
    </owl:Class>



    <!-- http://www.univ-tours.fr/ipato#Lettres_patentes -->

    <owl:Class rdf:about="http://www.univ-tours.fr/ipato#Lettres_patentes">
        <rdfs:subClassOf rdf:resource="http://erlangen-crm.org/current/E31_Document"/>
        <skos:definition xml:lang="fr">Terme générique pour désigner un acte de chancellerie, dans lequel souverain rend public une décision, un droit, un privilège, ou une action particulière.</skos:definition>
        <skos:prefLabel xml:lang="fr">Lettres patentes</skos:prefLabel>
    </owl:Class>



    <!-- http://www.univ-tours.fr/ipato#Minute_notariale -->

    <owl:Class rdf:about="http://www.univ-tours.fr/ipato#Minute_notariale">
        <rdfs:subClassOf rdf:resource="http://erlangen-crm.org/current/E31_Document"/>
        <skos:definition xml:lang="fr">Classe générique qui désigne tout acte issu de l&apos;écrit notarial.</skos:definition>
        <skos:prefLabel xml:lang="fr">Minute notariale</skos:prefLabel>
    </owl:Class>



    <!-- http://www.univ-tours.fr/ipato#Registre -->

    <owl:Class rdf:about="http://www.univ-tours.fr/ipato#Registre">
        <rdfs:subClassOf rdf:resource="http://erlangen-crm.org/current/E31_Document"/>
        <skos:definition xml:lang="fr">Classe générique pour désigner toute archive sous forme de cahier.</skos:definition>
        <skos:prefLabel xml:lang="fr">Registre</skos:prefLabel>
    </owl:Class>



    <!-- http://www.univ-tours.fr/ipato#Registre_de_délibération -->

    <owl:Class rdf:about="http://www.univ-tours.fr/ipato#Registre_de_délibération">
        <rdfs:subClassOf rdf:resource="http://www.univ-tours.fr/ipato#Registre"/>
        <skos:definition xml:lang="fr">Cahier qui enregistre et fait foi tous les actes de délibération d&apos;un corps de
ville, ainsi qu&apos;un certain nombre d&apos;acte complémentaires (lettres patentes ou closes, morceaux de comptabilité...)</skos:definition>
        <skos:prefLabel xml:lang="fr">Registre de délibération</skos:prefLabel>
    </owl:Class>



    <!-- http://www.univ-tours.fr/ipato#Registre_particulier_de_comptes -->

    <owl:Class rdf:about="http://www.univ-tours.fr/ipato#Registre_particulier_de_comptes">
        <rdfs:subClassOf rdf:resource="http://www.univ-tours.fr/ipato#Registre"/>
        <skos:definition xml:lang="fr">Cahier qui enregistre et fait foi tous les actes de la comptabilité d&apos;une autorité (un corps de ville, un chapitre...) pour une année ou une partie d&apos;année, ou pour seulement une partie des comptes (recettes, dépenses...)</skos:definition>
        <skos:prefLabel xml:lang="fr">Registre particulier de comptes</skos:prefLabel>
    </owl:Class>



    <!-- http://www.univ-tours.fr/ipato#Research_Area -->

    <owl:Class rdf:about="http://www.univ-tours.fr/ipato#Research_Area">
        <rdfs:comment>Testing class to be mapped to Eurovoc</rdfs:comment>
    </owl:Class>



    <!-- http://www.w3.org/ns/dcat#Catalog -->

    <owl:Class rdf:about="http://www.w3.org/ns/dcat#Catalog">
        <rdfs:subClassOf>
            <owl:Restriction>
                <owl:onProperty rdf:resource="http://www.w3.org/ns/dcat#dataset"/>
                <owl:someValuesFrom rdf:resource="http://www.w3.org/ns/dcat#Dataset"/>
            </owl:Restriction>
        </rdfs:subClassOf>
        <rdfs:subClassOf>
            <owl:Restriction>
                <owl:onProperty rdf:resource="http://purl.org/dc/terms/title"/>
                <owl:allValuesFrom rdf:resource="http://www.w3.org/2001/XMLSchema#string"/>
            </owl:Restriction>
        </rdfs:subClassOf>
        <rdfs:isDefinedBy rdf:datatype="http://www.w3.org/2001/XMLSchema#anyURI">https://www.w3.org/TR/vocab-dcat-2/</rdfs:isDefinedBy>
        <rdfs:label rdf:datatype="http://www.w3.org/2001/XMLSchema#string">Catalog</rdfs:label>
        <skos:definition rdf:datatype="http://www.w3.org/2001/XMLSchema#string">A curated collection of metadata about resources (e.g., datasets and data services in the context of a data catalog)</skos:definition>
        <skos:prefLabel xml:lang="en">Catalog</skos:prefLabel>
    </owl:Class>



    <!-- http://www.w3.org/ns/dcat#Dataset -->

    <owl:Class rdf:about="http://www.w3.org/ns/dcat#Dataset">
        <rdfs:subClassOf>
            <owl:Restriction>
                <owl:onProperty rdf:resource="http://purl.org/dc/terms/subject"/>
                <owl:someValuesFrom rdf:resource="http://www.univ-tours.fr/ipato#Research_Area"/>
            </owl:Restriction>
        </rdfs:subClassOf>
        <rdfs:subClassOf>
            <owl:Restriction>
                <owl:onProperty rdf:resource="http://www.univ-tours.fr/ipato#created_by"/>
                <owl:someValuesFrom rdf:resource="http://erlangen-crm.org/current/E39_Actor"/>
            </owl:Restriction>
        </rdfs:subClassOf>
        <rdfs:subClassOf>
            <owl:Restriction>
                <owl:onProperty rdf:resource="http://purl.org/dc/terms/language"/>
                <owl:allValuesFrom rdf:resource="http://erlangen-crm.org/current/E56_Language"/>
            </owl:Restriction>
        </rdfs:subClassOf>
        <rdfs:subClassOf>
            <owl:Restriction>
                <owl:onProperty rdf:resource="http://www.univ-tours.fr/ipato#dataCite_identifier"/>
                <owl:someValuesFrom rdf:resource="http://www.w3.org/2000/01/rdf-schema#Literal"/>
            </owl:Restriction>
        </rdfs:subClassOf>
        <rdfs:subClassOf>
            <owl:Restriction>
                <owl:onProperty rdf:resource="http://www.univ-tours.fr/ipato#dataIPAT_identifier"/>
                <owl:someValuesFrom rdf:resource="http://www.w3.org/2000/01/rdf-schema#Literal"/>
            </owl:Restriction>
        </rdfs:subClassOf>
        <rdfs:subClassOf>
            <owl:Restriction>
                <owl:onProperty rdf:resource="http://purl.org/dc/terms/description"/>
                <owl:allValuesFrom rdf:resource="http://www.w3.org/2001/XMLSchema#string"/>
            </owl:Restriction>
        </rdfs:subClassOf>
        <rdfs:subClassOf>
            <owl:Restriction>
                <owl:onProperty rdf:resource="http://purl.org/dc/terms/publisher"/>
                <owl:allValuesFrom rdf:resource="http://www.w3.org/2001/XMLSchema#string"/>
            </owl:Restriction>
        </rdfs:subClassOf>
        <rdfs:subClassOf>
            <owl:Restriction>
                <owl:onProperty rdf:resource="http://purl.org/dc/terms/rights"/>
                <owl:allValuesFrom rdf:resource="http://www.w3.org/2001/XMLSchema#string"/>
            </owl:Restriction>
        </rdfs:subClassOf>
        <rdfs:subClassOf>
            <owl:Restriction>
                <owl:onProperty rdf:resource="http://purl.org/dc/terms/title"/>
                <owl:allValuesFrom rdf:resource="http://www.w3.org/2001/XMLSchema#string"/>
            </owl:Restriction>
        </rdfs:subClassOf>
        <rdfs:isDefinedBy rdf:datatype="http://www.w3.org/2001/XMLSchema#anyURI">https://www.w3.org/TR/vocab-dcat-2/</rdfs:isDefinedBy>
        <rdfs:label xml:lang="en">Dataset</rdfs:label>
        <skos:definition rdf:datatype="http://www.w3.org/2001/XMLSchema#string">A collection of data, published or curated by a single agent, and available for access or download in one or more representations.</skos:definition>
        <skos:prefLabel xml:lang="en">Dataset</skos:prefLabel>
    </owl:Class>



    <!-- http://xmlns.com/foaf/0.1/Agent -->

    <owl:Class rdf:about="http://xmlns.com/foaf/0.1/Agent">
        <rdfs:subClassOf rdf:resource="http://erlangen-crm.org/current/E77_Persistent_Item"/>
    </owl:Class>



    <!-- http://xmlns.com/foaf/0.1/Group -->

    <owl:Class rdf:about="http://xmlns.com/foaf/0.1/Group">
        <rdfs:subClassOf rdf:resource="http://erlangen-crm.org/current/E39_Actor"/>
    </owl:Class>



    <!-- http://xmlns.com/foaf/0.1/Organization -->

    <owl:Class rdf:about="http://xmlns.com/foaf/0.1/Organization">
        <rdfs:subClassOf rdf:resource="http://erlangen-crm.org/current/E39_Actor"/>
    </owl:Class>



    <!-- http://xmlns.com/foaf/0.1/Person -->

    <owl:Class rdf:about="http://xmlns.com/foaf/0.1/Person">
        <rdfs:subClassOf rdf:resource="http://erlangen-crm.org/current/E20_Biological_Object"/>
        <rdfs:subClassOf>
            <owl:Restriction>
                <owl:onProperty rdf:resource="http://www.univ-tours.fr/ipato#has_role"/>
                <owl:allValuesFrom rdf:resource="http://id.loc.gov/ontologies/bibframe/Role"/>
            </owl:Restriction>
        </rdfs:subClassOf>
        <rdfs:subClassOf>
            <owl:Restriction>
                <owl:onProperty rdf:resource="http://xmlns.com/foaf/0.1/firstName"/>
                <owl:allValuesFrom rdf:resource="http://www.w3.org/2001/XMLSchema#string"/>
            </owl:Restriction>
        </rdfs:subClassOf>
        <rdfs:subClassOf>
            <owl:Restriction>
                <owl:onProperty rdf:resource="http://xmlns.com/foaf/0.1/lastName"/>
                <owl:allValuesFrom rdf:resource="http://www.w3.org/2001/XMLSchema#string"/>
            </owl:Restriction>
        </rdfs:subClassOf>
        <rdfs:subClassOf>
            <owl:Restriction>
                <owl:onProperty rdf:resource="http://xmlns.com/foaf/0.1/mbox"/>
                <owl:allValuesFrom rdf:resource="http://www.w3.org/2001/XMLSchema#anyURI"/>
            </owl:Restriction>
        </rdfs:subClassOf>
        <rdfs:subClassOf>
            <owl:Restriction>
                <owl:onProperty rdf:resource="http://xmlns.com/foaf/0.1/name"/>
                <owl:allValuesFrom rdf:resource="http://www.w3.org/2001/XMLSchema#string"/>
            </owl:Restriction>
        </rdfs:subClassOf>
    </owl:Class>



    <!-- http://xmlns.com/foaf/0.1/Project -->

    <owl:Class rdf:about="http://xmlns.com/foaf/0.1/Project">
        <rdfs:subClassOf>
            <owl:Restriction>
                <owl:onProperty rdf:resource="http://purl.org/cerif/frapo/hasFundingAgency"/>
                <owl:someValuesFrom rdf:resource="http://www.univ-tours.fr/ipato#FundingAgency"/>
            </owl:Restriction>
        </rdfs:subClassOf>
        <rdfs:subClassOf>
            <owl:Restriction>
                <owl:onProperty rdf:resource="http://www.univ-tours.fr/ipato#has_catalog"/>
                <owl:someValuesFrom rdf:resource="http://www.w3.org/ns/dcat#Catalog"/>
            </owl:Restriction>
        </rdfs:subClassOf>
        <rdfs:subClassOf>
            <owl:Restriction>
                <owl:onProperty rdf:resource="http://www.univ-tours.fr/ipato#has_project_participant"/>
                <owl:someValuesFrom rdf:resource="http://erlangen-crm.org/current/E39_Actor"/>
            </owl:Restriction>
        </rdfs:subClassOf>
        <rdfs:subClassOf>
            <owl:Restriction>
                <owl:onProperty rdf:resource="http://www.univ-tours.fr/ipato#has_research_area"/>
                <owl:someValuesFrom rdf:resource="http://www.univ-tours.fr/ipato#Research_Area"/>
            </owl:Restriction>
        </rdfs:subClassOf>
        <rdfs:subClassOf>
            <owl:Restriction>
                <owl:onProperty rdf:resource="http://www.univ-tours.fr/ipato#is_about"/>
                <owl:someValuesFrom rdf:resource="http://erlangen-crm.org/current/E1_CRM_Entity"/>
            </owl:Restriction>
        </rdfs:subClassOf>
        <rdfs:subClassOf>
            <owl:Restriction>
                <owl:onProperty rdf:resource="http://www.univ-tours.fr/ipato#is_coordinated_by"/>
                <owl:someValuesFrom rdf:resource="http://erlangen-crm.org/current/E21_Person"/>
            </owl:Restriction>
        </rdfs:subClassOf>
        <rdfs:subClassOf>
            <owl:Restriction>
                <owl:onProperty rdf:resource="http://www.univ-tours.fr/ipato#is_associated_to"/>
                <owl:allValuesFrom rdf:resource="http://xmlns.com/foaf/0.1/Group"/>
            </owl:Restriction>
        </rdfs:subClassOf>
        <rdfs:subClassOf>
            <owl:Restriction>
                <owl:onProperty rdf:resource="http://purl.org/dc/terms/title"/>
                <owl:allValuesFrom rdf:resource="http://www.w3.org/2001/XMLSchema#string"/>
            </owl:Restriction>
        </rdfs:subClassOf>
        <rdfs:label xml:lang="en">Project</rdfs:label>
    </owl:Class>



    <!--
    ///////////////////////////////////////////////////////////////////////////////////////
    //
    // Individuals
    //
    ///////////////////////////////////////////////////////////////////////////////////////
     -->




    <!-- http://www.univ-tours.fr/ipato#Accord -->

    <owl:NamedIndividual rdf:about="http://www.univ-tours.fr/ipato#Accord">
        <rdf:type rdf:resource="http://www.univ-tours.fr/ipato#Forme_De_Acte"/>
        <skos:altLabel xml:lang="en">Contract</skos:altLabel>
        <skos:definition xml:lang="en">A deed by which at least two individuals, acting in their own name or as representatives of a group of persons, agree on a negotiation of any kind (commercial, financial, legal, etc.).</skos:definition>
        <skos:definition xml:lang="fr">Acte par lequel au moins deux individus, agissant en leur nom propre ou comme représentants d&apos;un groupe de personnes, s&apos;entendent sur une négociation de quelque nature qu&apos;elle soit (commerciale, financière, juridique, etc.).</skos:definition>
        <skos:prefLabel xml:lang="fr">Accord</skos:prefLabel>
    </owl:NamedIndividual>



    <!-- http://www.univ-tours.fr/ipato#Acte_de_notoriété -->

    <owl:NamedIndividual rdf:about="http://www.univ-tours.fr/ipato#Acte_de_notoriété">
        <rdf:type rdf:resource="http://www.univ-tours.fr/ipato#Forme_De_Acte"/>
        <skos:altLabel xml:lang="en">Act of renoun</skos:altLabel>
        <skos:altLabel xml:lang="en">Deed of notoriety</skos:altLabel>
        <skos:definition xml:lang="fr">Témoignage écrit par lequel une ou plusieurs personnes attestent un fait, un statut individuel, par exemple, comme connu et avéré, faute d&apos;une preuve écrite.</skos:definition>
        <skos:definition xml:lang="en">Written testimony by which one or more persons attest a fact, or an individual status, for example, as known and proven, in the absence of written evidence.</skos:definition>
        <skos:prefLabel xml:lang="fr">Acte de notoriété</skos:prefLabel>
    </owl:NamedIndividual>



    <!-- http://www.univ-tours.fr/ipato#Assignation_à_comparaître -->

    <owl:NamedIndividual rdf:about="http://www.univ-tours.fr/ipato#Assignation_à_comparaître">
        <rdf:type rdf:resource="http://www.univ-tours.fr/ipato#Forme_De_Acte"/>
        <skos:altLabel xml:lang="en">Summons to appear</skos:altLabel>
        <skos:definition xml:lang="en">A deed by which a person is formally summoned before a legal body, whether local, in the context of seigniorial justice for example, or at the level of the kingdom in the case of a summons to appear before a Parliament.</skos:definition>
        <skos:definition xml:lang="fr">Acte par lequel une personne est formellement convoquée devant une instance juridique qu&apos;elle soit locale, dans le cadre de la justice seigneuriale par exemple, ou à l&apos;échelle du royaume s&apos;il s&apos;agit d&apos;une convocation devant un Parlement.</skos:definition>
        <skos:prefLabel xml:lang="fr">Assignation à comparaître</skos:prefLabel>
    </owl:NamedIndividual>



    <!-- http://www.univ-tours.fr/ipato#Association -->

    <owl:NamedIndividual rdf:about="http://www.univ-tours.fr/ipato#Association">
        <rdf:type rdf:resource="http://www.univ-tours.fr/ipato#Forme_De_Acte"/>
        <skos:altLabel xml:lang="en">Collaboration</skos:altLabel>
        <skos:definition xml:lang="en">Acte par lequel au moins deux individus mettent en commun des moyens fonciers et/ou matériels pour la réalisation d&apos;une entreprise, le plus souvent commerciale.</skos:definition>
        <skos:definition xml:lang="en">Deed by which at least two individuals pool property and/or material resources to carry out a venture, most often a commercial one.</skos:definition>
        <skos:prefLabel xml:lang="fr">Association</skos:prefLabel>
    </owl:NamedIndividual>



    <!-- http://www.univ-tours.fr/ipato#Aveu -->

    <owl:NamedIndividual rdf:about="http://www.univ-tours.fr/ipato#Aveu">
        <rdf:type rdf:resource="http://www.univ-tours.fr/ipato#Forme_De_Acte"/>
        <skos:altLabel xml:lang="en">Declaration</skos:altLabel>
        <skos:definition xml:lang="en">Declaration of possession of land or real estate attached to a fief formulated by a vassal to his suzerain.</skos:definition>
        <skos:definition xml:lang="en">Déclaration de possession d&apos;un bien foncier ou immobilier rattaché à un fief formulée par un vassal à son suzerain.</skos:definition>
        <skos:prefLabel xml:lang="fr">Aveu</skos:prefLabel>
    </owl:NamedIndividual>



    <!-- http://www.univ-tours.fr/ipato#Bail -->

    <owl:NamedIndividual rdf:about="http://www.univ-tours.fr/ipato#Bail">
        <rdf:type rdf:resource="http://www.univ-tours.fr/ipato#Forme_De_Acte"/>
        <skos:altLabel xml:lang="en">Lease</skos:altLabel>
        <skos:definition xml:lang="en">Contract by which one of the parties (called lessor), landowner or real estate owner, undertakes to transfer the occupation of his movable or immovable property to a third party (the lessee) for a limited period of time in return for the payment of a rent.</skos:definition>
        <skos:definition xml:lang="fr">Contrat par lequel l&apos;une des parties (appelée bailleur), propriétaire foncier ou immobilier, s&apos;engage à céder pour un temps délimité, l&apos;occupation de son bien mobilier ou immobilier à une tierce personne (le prenneur) moyennant le versement d&apos;un loyer.</skos:definition>
        <skos:prefLabel xml:lang="fr">Bail</skos:prefLabel>
    </owl:NamedIndividual>



    <!-- http://www.univ-tours.fr/ipato#Bail_perpétuel -->

    <owl:NamedIndividual rdf:about="http://www.univ-tours.fr/ipato#Bail_perpétuel">
        <rdf:type rdf:resource="http://www.univ-tours.fr/ipato#Forme_De_Acte"/>
        <skos:definition xml:lang="fr">Contrat illimité dans le temps par lequel l&apos;une des parties (appelée bailleur), propriétaire foncier ou immobilier, s&apos;engage à céder l&apos;occupation d&apos;un bien à une tierce personne (le prenneur) et qui définit les modalités financières et matérielles de l&apos;occupation et de la gestion du bien.</skos:definition>
        <skos:prefLabel xml:lang="fr">Bail perpétuel</skos:prefLabel>
    </owl:NamedIndividual>



    <!-- http://www.univ-tours.fr/ipato#Bail_à_cens -->

    <owl:NamedIndividual rdf:about="http://www.univ-tours.fr/ipato#Bail_à_cens">
        <rdf:type rdf:resource="http://www.univ-tours.fr/ipato#Forme_De_Acte"/>
        <skos:altLabel xml:lang="en">Cens lease</skos:altLabel>
        <skos:definition xml:lang="en">Contract by which one of the parties (called the lessor), owner of land or property, undertakes to transfer the occupation of his property to a third person (the lessee) in return for the payment of a cens.</skos:definition>
        <skos:definition xml:lang="fr">Contrat par lequel l&apos;une des parties (appelée bailleur), propriétaire foncier ou immobilier, s&apos;engage à céder l&apos;occupation de son bien à une tierce personne (le prenneur) moyennant le versement d&apos;un cens.</skos:definition>
        <skos:prefLabel xml:lang="fr">Bail à cens</skos:prefLabel>
    </owl:NamedIndividual>



    <!-- http://www.univ-tours.fr/ipato#Bail_à_ferme -->

    <owl:NamedIndividual rdf:about="http://www.univ-tours.fr/ipato#Bail_à_ferme">
        <rdf:type rdf:resource="http://www.univ-tours.fr/ipato#Forme_De_Acte"/>
        <skos:definition xml:lang="en">Contract by which one of the parties (called the lessor), a land or property owner, undertakes to transfer the occupation of a property placed under the lease system to a third party (the lessee) and which defines the financial and material terms and conditions for the occupation and management of the property.</skos:definition>
        <skos:definition xml:lang="fr">Contrat par lequel l&apos;une des parties (appelée bailleur), propriétaire foncier ou immobilier, s&apos;engage à céder l&apos;occupation d&apos;un bien placé sous le régime de l&apos;affermage à une tierce personne (le prenneur) et qui définit les modalités financières et matérielles de l&apos;occupation et de la gestion du bien.</skos:definition>
        <skos:prefLabel xml:lang="fr">Bail à ferme</skos:prefLabel>
    </owl:NamedIndividual>



    <!-- http://www.univ-tours.fr/ipato#Bail_à_métairie -->

    <owl:NamedIndividual rdf:about="http://www.univ-tours.fr/ipato#Bail_à_métairie">
        <rdf:type rdf:resource="http://www.univ-tours.fr/ipato#Forme_De_Acte"/>
        <skos:definition xml:lang="fr">Contrat par lequel l&apos;une des parties (appelée bailleur), propriétaire foncier ou immobilier, s&apos;engage à céder l&apos;occupation d&apos;un bien placé sous le régime de la métairie à une tierce personne (le prenneur) et qui définit les modalités financières et matérielles de l&apos;occupation et de la gestion du bien.</skos:definition>
        <skos:prefLabel xml:lang="fr">Bail à métairie</skos:prefLabel>
    </owl:NamedIndividual>



    <!-- http://www.univ-tours.fr/ipato#Bail_à_rente -->

    <owl:NamedIndividual rdf:about="http://www.univ-tours.fr/ipato#Bail_à_rente">
        <rdf:type rdf:resource="http://www.univ-tours.fr/ipato#Forme_De_Acte"/>
        <skos:definition xml:lang="fr">Contrat d’aliénation d’un immeuble (généralement une terre ou une maison) sur lequel le bailleur se réserve le droit de percevoir une partie des revenus, sous la forme d’une redevance (la rente) annuelle et perpétuelle</skos:definition>
        <skos:prefLabel xml:lang="fr">Bail à rente</skos:prefLabel>
    </owl:NamedIndividual>



    <!-- http://www.univ-tours.fr/ipato#Cautionnement -->

    <owl:NamedIndividual rdf:about="http://www.univ-tours.fr/ipato#Cautionnement">
        <rdf:type rdf:resource="http://www.univ-tours.fr/ipato#Forme_De_Acte"/>
        <skos:definition xml:lang="fr">Acte par lequel une personne se porte financièrement garante d&apos;une seconde, pour une somme précise et définie, dans le cadre d&apos;une transaction commerciale, le plus souvent.</skos:definition>
        <skos:prefLabel xml:lang="fr">Cautionnement</skos:prefLabel>
    </owl:NamedIndividual>



    <!-- http://www.univ-tours.fr/ipato#Cession -->

    <owl:NamedIndividual rdf:about="http://www.univ-tours.fr/ipato#Cession">
        <rdf:type rdf:resource="http://www.univ-tours.fr/ipato#Forme_De_Acte"/>
        <skos:altLabel xml:lang="en">Transfer</skos:altLabel>
        <skos:definition xml:lang="fr">Acte par lequel une personne transfère gratuitement à une autre un bien foncier, un bien meuble ou immeuble, un ou plusieurs droits, etc.</skos:definition>
        <skos:prefLabel xml:lang="fr">Cession</skos:prefLabel>
    </owl:NamedIndividual>



    <!-- http://www.univ-tours.fr/ipato#Compte -->

    <owl:NamedIndividual rdf:about="http://www.univ-tours.fr/ipato#Compte">
        <rdf:type rdf:resource="http://www.univ-tours.fr/ipato#Forme_De_Acte"/>
        <skos:definition xml:lang="fr">Document qui liste de façon plus ou moins détaillée des sommes d&apos;argent reçues et/ou dépensées dans un cadre spécifique généralement précisée en début et qui sert à de sfins de vérification et de gestion comptable et financière.</skos:definition>
        <skos:prefLabel xml:lang="fr">Compte</skos:prefLabel>
    </owl:NamedIndividual>



    <!-- http://www.univ-tours.fr/ipato#Consentement -->

    <owl:NamedIndividual rdf:about="http://www.univ-tours.fr/ipato#Consentement">
        <rdf:type rdf:resource="http://www.univ-tours.fr/ipato#Forme_De_Acte"/>
        <skos:definition xml:lang="fr">Acte par lequel une personne accepte officiellement une transaction, un accord, etc.</skos:definition>
        <skos:prefLabel xml:lang="fr">Consentement</skos:prefLabel>
    </owl:NamedIndividual>



    <!-- http://www.univ-tours.fr/ipato#Constitution_de_rente -->

    <owl:NamedIndividual rdf:about="http://www.univ-tours.fr/ipato#Constitution_de_rente">
        <rdf:type rdf:resource="http://www.univ-tours.fr/ipato#Forme_De_Acte"/>
        <skos:definition xml:lang="fr">Acte par lequel une personne assujetti un bien foncier ou immobilier à une rente, c&apos;est-à-dire à une redevance généralement annuelle due par l&apos;occupant du bien à son propriétaire.</skos:definition>
        <skos:prefLabel xml:lang="fr">Constitution de rente</skos:prefLabel>
    </owl:NamedIndividual>



    <!-- http://www.univ-tours.fr/ipato#Contrat -->

    <owl:NamedIndividual rdf:about="http://www.univ-tours.fr/ipato#Contrat">
        <rdf:type rdf:resource="http://www.univ-tours.fr/ipato#Forme_De_Acte"/>
        <skos:altLabel xml:lang="en">Contract</skos:altLabel>
        <skos:definition xml:lang="fr">Acte juridique établissant les modalités de toutes transaction ou de relation entre personnes.</skos:definition>
        <skos:prefLabel xml:lang="fr">Contrat</skos:prefLabel>
    </owl:NamedIndividual>



    <!-- http://www.univ-tours.fr/ipato#Contrat_apprentissage -->

    <owl:NamedIndividual rdf:about="http://www.univ-tours.fr/ipato#Contrat_apprentissage">
        <rdf:type rdf:resource="http://www.univ-tours.fr/ipato#Forme_De_Acte"/>
        <skos:altLabel xml:lang="en">Apprenticeship contract</skos:altLabel>
        <skos:definition xml:lang="fr">Acte établissant les modalités temporelles, morales, matérielles et financières de la prise en charge par un artisan établi d&apos;un apprenti.</skos:definition>
        <skos:prefLabel xml:lang="fr">Contrat d&apos;apprentissage</skos:prefLabel>
    </owl:NamedIndividual>



    <!-- http://www.univ-tours.fr/ipato#Contrat_mariage -->

    <owl:NamedIndividual rdf:about="http://www.univ-tours.fr/ipato#Contrat_mariage">
        <rdf:type rdf:resource="http://www.univ-tours.fr/ipato#Forme_De_Acte"/>
        <skos:altLabel xml:lang="en">Marriage contract</skos:altLabel>
        <skos:definition xml:lang="en">Acte établissant les modalités morales, matérielles et financières d&apos;une union maritale entre deux personnes.</skos:definition>
        <skos:prefLabel xml:lang="fr">Contrat de mariage</skos:prefLabel>
    </owl:NamedIndividual>



    <!-- http://www.univ-tours.fr/ipato#Correspondance_administrative -->

    <owl:NamedIndividual rdf:about="http://www.univ-tours.fr/ipato#Correspondance_administrative">
        <rdf:type rdf:resource="http://www.univ-tours.fr/ipato#Forme_De_Acte"/>
        <skos:altLabel xml:lang="en">Administrative correspondance</skos:altLabel>
        <skos:altLabel xml:lang="fr">Ensemble des échanges épistolaires entre des personnes d&apos;une même autorité administrative pour le bon fonctionnement de l&apos;autorité en question.</skos:altLabel>
        <skos:prefLabel xml:lang="fr">Correspondance administrative</skos:prefLabel>
    </owl:NamedIndividual>



    <!-- http://www.univ-tours.fr/ipato#Correspondance_politique -->

    <owl:NamedIndividual rdf:about="http://www.univ-tours.fr/ipato#Correspondance_politique">
        <rdf:type rdf:resource="http://www.univ-tours.fr/ipato#Forme_De_Acte"/>
        <skos:altLabel xml:lang="en">Political correspondance</skos:altLabel>
        <skos:definition xml:lang="fr">Ensemble des échanges épistolaires qui ont eu lieu entre des autorités politiques différentes via leurs représentants.</skos:definition>
        <skos:prefLabel xml:lang="fr">Correspondance politique</skos:prefLabel>
    </owl:NamedIndividual>



    <!-- http://www.univ-tours.fr/ipato#Don -->

    <owl:NamedIndividual rdf:about="http://www.univ-tours.fr/ipato#Don">
        <rdf:type rdf:resource="http://www.univ-tours.fr/ipato#Forme_De_Acte"/>
        <skos:altLabel xml:lang="en">Deed of gift</skos:altLabel>
        <skos:definition xml:lang="fr">Acte témoignant d&apos;une donation.</skos:definition>
        <skos:prefLabel xml:lang="fr">Don</skos:prefLabel>
    </owl:NamedIndividual>



    <!-- http://www.univ-tours.fr/ipato#Donation -->

    <owl:NamedIndividual rdf:about="http://www.univ-tours.fr/ipato#Donation">
        <rdf:type rdf:resource="http://www.univ-tours.fr/ipato#Forme_De_Acte"/>
        <skos:definition xml:lang="fr">Acte par lequel une personne cède de façon gratuite à une autre personne ou à un ensemble de personnes un bien, des droits, une charge, etc.</skos:definition>
        <skos:prefLabel xml:lang="fr">Donation</skos:prefLabel>
    </owl:NamedIndividual>



    <!-- http://www.univ-tours.fr/ipato#Délibération_de_corps_de_ville -->

    <owl:NamedIndividual rdf:about="http://www.univ-tours.fr/ipato#Délibération_de_corps_de_ville">
        <rdf:type rdf:resource="http://www.univ-tours.fr/ipato#Forme_De_Acte"/>
        <skos:definition xml:lang="fr">Ensemble des débats et des prises de décision qui ont lieu au sein d&apos;une autorité municipale à l&apos;occasion des conseils du corps de ville.</skos:definition>
        <skos:prefLabel xml:lang="fr">Délibération de corps de ville</skos:prefLabel>
    </owl:NamedIndividual>



    <!-- http://www.univ-tours.fr/ipato#Déposition -->

    <owl:NamedIndividual rdf:about="http://www.univ-tours.fr/ipato#Déposition">
        <rdf:type rdf:resource="http://www.univ-tours.fr/ipato#Forme_De_Acte"/>
        <skos:definition xml:lang="fr">Acte par lequel une personne fournit à une autorité judiciaire ou juridique son témoignange sur un fait.</skos:definition>
        <skos:prefLabel xml:lang="fr">Déposition</skos:prefLabel>
    </owl:NamedIndividual>



    <!-- http://www.univ-tours.fr/ipato#Echange -->

    <owl:NamedIndividual rdf:about="http://www.univ-tours.fr/ipato#Echange">
        <rdf:type rdf:resource="http://www.univ-tours.fr/ipato#Forme_De_Acte"/>
        <skos:definition xml:lang="fr">Transaction par laquelle deux personnes se donnent mutuellement un ou plusieurs biens ou droits fonciers, mobiliers et/ou immobiliers de valeurs équivalentes, sans engagement de numéraire sauf dans le cas d&apos;une compensation en cas d&apos;inégalité de valeur.</skos:definition>
        <skos:prefLabel xml:lang="fr">Echange</skos:prefLabel>
    </owl:NamedIndividual>



    <!-- http://www.univ-tours.fr/ipato#Ecrits_du_for_privé -->

    <owl:NamedIndividual rdf:about="http://www.univ-tours.fr/ipato#Ecrits_du_for_privé">
        <rdf:type rdf:resource="http://www.univ-tours.fr/ipato#Forme_De_Acte"/>
        <skos:definition xml:lang="fr">Document non officiel livrant de sinformations sur l&apos;individualité de la personne rédactrice.</skos:definition>
        <skos:prefLabel xml:lang="fr">Ecrits du for privé</skos:prefLabel>
    </owl:NamedIndividual>



    <!-- http://www.univ-tours.fr/ipato#Fondation -->

    <owl:NamedIndividual rdf:about="http://www.univ-tours.fr/ipato#Fondation">
        <rdf:type rdf:resource="http://www.univ-tours.fr/ipato#Forme_De_Acte"/>
        <skos:definition xml:lang="fr">Document par lequel une personne commande à une communauté religieuse régulière ou séculière la prononciation d&apos;une ou plusieurs messes, le plus souvent pour le salut post mortem de son âme et/ou pour le souvenir de ses proches défunts, en échange d&apos;une contrepartie financière pouvant prendre plusieurs formes.</skos:definition>
        <skos:prefLabel xml:lang="fr">Fondation</skos:prefLabel>
    </owl:NamedIndividual>



    <!-- http://www.univ-tours.fr/ipato#France -->

    <owl:NamedIndividual rdf:about="http://www.univ-tours.fr/ipato#France">
        <rdf:type rdf:resource="http://dbpedia.org/ontology/Country"/>
    </owl:NamedIndividual>



    <!-- http://www.univ-tours.fr/ipato#Inventaire_après_décès -->

    <owl:NamedIndividual rdf:about="http://www.univ-tours.fr/ipato#Inventaire_après_décès">
        <rdf:type rdf:resource="http://www.univ-tours.fr/ipato#Forme_De_Acte"/>
        <skos:definition xml:lang="fr">Liste des biens mobiliers, le plus souvent, détenus par une personne décédée dans sa ou ses résidences à des fins de partage ultérieur.</skos:definition>
        <skos:prefLabel xml:lang="fr">Inventaire après décès</skos:prefLabel>
    </owl:NamedIndividual>



    <!-- http://www.univ-tours.fr/ipato#Leg -->

    <owl:NamedIndividual rdf:about="http://www.univ-tours.fr/ipato#Leg">
        <rdf:type rdf:resource="http://www.univ-tours.fr/ipato#Forme_De_Acte"/>
        <skos:definition xml:lang="fr">Donation régie par prédisposition testamentaire.</skos:definition>
        <skos:prefLabel xml:lang="fr">Leg</skos:prefLabel>
    </owl:NamedIndividual>



    <!-- http://www.univ-tours.fr/ipato#Mandement_de_paiement -->

    <owl:NamedIndividual rdf:about="http://www.univ-tours.fr/ipato#Mandement_de_paiement">
        <rdf:type rdf:resource="http://www.univ-tours.fr/ipato#Forme_De_Acte"/>
        <skos:definition xml:lang="fr">Acte par lequel une personne ordonne le payement d&apos;une somme précise.</skos:definition>
        <skos:prefLabel xml:lang="fr">Mandement de paiement</skos:prefLabel>
    </owl:NamedIndividual>



    <!-- http://www.univ-tours.fr/ipato#Marchant -->

    <owl:NamedIndividual rdf:about="http://www.univ-tours.fr/ipato#Marchant">
        <rdf:type rdf:resource="http://erlangen-crm.org/current/E21_Person"/>
        <has_role rdf:resource="http://www.univ-tours.fr/ipato#Notary"/>
        <has_role rdf:resource="http://www.univ-tours.fr/ipato#Royal_Secretary"/>
    </owl:NamedIndividual>



    <!-- http://www.univ-tours.fr/ipato#Marché -->

    <owl:NamedIndividual rdf:about="http://www.univ-tours.fr/ipato#Marché">
        <rdf:type rdf:resource="http://www.univ-tours.fr/ipato#Forme_De_Acte"/>
        <skos:definition xml:lang="fr">Acte par lequel une personne passe commande auprès d&apos;un artiste ou d&apos;un artisan.</skos:definition>
        <skos:prefLabel xml:lang="fr">Marché</skos:prefLabel>
    </owl:NamedIndividual>



    <!-- http://www.univ-tours.fr/ipato#Millimetre -->

    <owl:NamedIndividual rdf:about="http://www.univ-tours.fr/ipato#Millimetre">
        <rdf:type rdf:resource="http://erlangen-crm.org/current/E58_Measurement_Unit"/>
        <skos:altLabel>mm</skos:altLabel>
        <skos:prefLabel xml:lang="en">millimetre</skos:prefLabel>
    </owl:NamedIndividual>



    <!-- http://www.univ-tours.fr/ipato#Métayage -->

    <owl:NamedIndividual rdf:about="http://www.univ-tours.fr/ipato#Métayage">
        <rdf:type rdf:resource="http://www.univ-tours.fr/ipato#Forme_De_Acte"/>
        <skos:definition xml:lang="fr">Acte par lequel un propriétaire foncier place la gestion agricole de sa terre sous le régime de la métairie.</skos:definition>
        <skos:prefLabel xml:lang="fr">Métayage</skos:prefLabel>
    </owl:NamedIndividual>



    <!-- http://www.univ-tours.fr/ipato#Notary -->

    <owl:NamedIndividual rdf:about="http://www.univ-tours.fr/ipato#Notary">
        <rdf:type rdf:resource="http://id.loc.gov/ontologies/bibframe/Role"/>
    </owl:NamedIndividual>



    <!-- http://www.univ-tours.fr/ipato#Obligation -->

    <owl:NamedIndividual rdf:about="http://www.univ-tours.fr/ipato#Obligation">
        <rdf:type rdf:resource="http://www.univ-tours.fr/ipato#Forme_De_Acte"/>
        <skos:definition xml:lang="fr">Acte par lequel une personne s&apos;engage officiellement à peyer une somme d&apos;argent définie en prenant un bien ou plusieurs biens fonciers ou immeubles de valeur équivalente à la dette comme garantie de payement.</skos:definition>
        <skos:prefLabel xml:lang="fr">Obligation</skos:prefLabel>
    </owl:NamedIndividual>



    <!-- http://www.univ-tours.fr/ipato#Ordonnance -->

    <owl:NamedIndividual rdf:about="http://www.univ-tours.fr/ipato#Ordonnance">
        <rdf:type rdf:resource="http://www.univ-tours.fr/ipato#Forme_De_Acte"/>
        <skos:definition xml:lang="fr">Acte de chancellerie qui étend les effets d&apos;une délibération royale ou princière à tout un territoire.</skos:definition>
        <skos:prefLabel xml:lang="fr">Ordonnance</skos:prefLabel>
    </owl:NamedIndividual>



    <!-- http://www.univ-tours.fr/ipato#Partage -->

    <owl:NamedIndividual rdf:about="http://www.univ-tours.fr/ipato#Partage">
        <rdf:type rdf:resource="http://www.univ-tours.fr/ipato#Forme_De_Acte"/>
        <skos:definition xml:lang="fr">Acte par lequel au moins deux personnes se divisent un bien foncier ou immobilier, ou un ensemble de bien comme, par exemple, dans le cadre d&apos;une succession.</skos:definition>
        <skos:prefLabel xml:lang="fr">Partage</skos:prefLabel>
    </owl:NamedIndividual>



    <!-- http://www.univ-tours.fr/ipato#Plaidoyer -->

    <owl:NamedIndividual rdf:about="http://www.univ-tours.fr/ipato#Plaidoyer">
        <rdf:type rdf:resource="http://www.univ-tours.fr/ipato#Forme_De_Acte"/>
        <skos:definition xml:lang="fr">Acte établissant l&apos;argumentaire d&apos;une personne devant une instance juridique.</skos:definition>
        <skos:prefLabel xml:lang="fr">Plaidoyer</skos:prefLabel>
    </owl:NamedIndividual>



    <!-- http://www.univ-tours.fr/ipato#Procuration -->

    <owl:NamedIndividual rdf:about="http://www.univ-tours.fr/ipato#Procuration">
        <rdf:type rdf:resource="http://www.univ-tours.fr/ipato#Forme_De_Acte"/>
        <skos:definition xml:lang="fr">Acte par lequel une personne délègue à une autre personne tout ou partie de ses droits pour la représenter devant toute instance officielle.</skos:definition>
        <skos:prefLabel xml:lang="fr">Procuration</skos:prefLabel>
    </owl:NamedIndividual>



    <!-- http://www.univ-tours.fr/ipato#Procès-verbal -->

    <owl:NamedIndividual rdf:about="http://www.univ-tours.fr/ipato#Procès-verbal">
        <rdf:type rdf:resource="http://www.univ-tours.fr/ipato#Forme_De_Acte"/>
        <skos:prefLabel xml:lang="fr">Procès-verbal</skos:prefLabel>
    </owl:NamedIndividual>



    <!-- http://www.univ-tours.fr/ipato#Prolongation_de_réméré -->

    <owl:NamedIndividual rdf:about="http://www.univ-tours.fr/ipato#Prolongation_de_réméré">
        <rdf:type rdf:resource="http://www.univ-tours.fr/ipato#Forme_De_Acte"/>
        <skos:definition xml:lang="fr">Acte par lequel l&apos;acheteur d&apos;un bien, le plus souvent foncier, accorde à son vendeur l&apos;extension dans le temps de sa faculté de récupérer de façon onéreuse le bien vendu, au-delà de la clause initialement contractualisée.</skos:definition>
        <skos:prefLabel xml:lang="fr">Prolongation de réméré</skos:prefLabel>
    </owl:NamedIndividual>



    <!-- http://www.univ-tours.fr/ipato#Promesse -->

    <owl:NamedIndividual rdf:about="http://www.univ-tours.fr/ipato#Promesse">
        <rdf:type rdf:resource="http://www.univ-tours.fr/ipato#Forme_De_Acte"/>
        <skos:definition xml:lang="fr">Acte par lequel une personne s&apos;engage officiellement auprès d&apos;une autre personne pour une transaction gratuite ou onéreuse.</skos:definition>
        <skos:prefLabel xml:lang="fr">Promesse</skos:prefLabel>
    </owl:NamedIndividual>



    <!-- http://www.univ-tours.fr/ipato#Promesse_de_vente -->

    <owl:NamedIndividual rdf:about="http://www.univ-tours.fr/ipato#Promesse_de_vente">
        <rdf:type rdf:resource="http://www.univ-tours.fr/ipato#Forme_De_Acte"/>
        <skos:definition xml:lang="fr">Acte par lequel un vendeur s&apos;engage auprès d&apos;un acheteur à lui vendre un bien immobilier, principalement.</skos:definition>
        <skos:prefLabel xml:lang="fr">Promesse de vente</skos:prefLabel>
    </owl:NamedIndividual>



    <!-- http://www.univ-tours.fr/ipato#Provision_office -->

    <owl:NamedIndividual rdf:about="http://www.univ-tours.fr/ipato#Provision_office">
        <rdf:type rdf:resource="http://www.univ-tours.fr/ipato#Forme_De_Acte"/>
        <skos:definition xml:lang="fr">Acte délivré par me pouvoir royal par lequel une personne est officiellement investie d&apos;un charge ou d&apos;une fonction délivrée</skos:definition>
        <skos:prefLabel xml:lang="fr">Provision d&apos;office</skos:prefLabel>
    </owl:NamedIndividual>



    <!-- http://www.univ-tours.fr/ipato#Quittance -->

    <owl:NamedIndividual rdf:about="http://www.univ-tours.fr/ipato#Quittance">
        <rdf:type rdf:resource="http://www.univ-tours.fr/ipato#Forme_De_Acte"/>
        <skos:definition xml:lang="fr">Document attestant du verseent ou de la réception d&apos;une somme d&apos;argent, le plus souvent.</skos:definition>
        <skos:prefLabel xml:lang="fr">Quittance</skos:prefLabel>
    </owl:NamedIndividual>



    <!-- http://www.univ-tours.fr/ipato#Ratification -->

    <owl:NamedIndividual rdf:about="http://www.univ-tours.fr/ipato#Ratification">
        <rdf:type rdf:resource="http://www.univ-tours.fr/ipato#Forme_De_Acte"/>
        <skos:definition xml:lang="fr">Acte par lequel une personne valide la signature d&apos;un acte initialement contracté par une tierce personne la représentant auprès d&apos;une instance juridique.</skos:definition>
        <skos:prefLabel xml:lang="fr">Ratification</skos:prefLabel>
    </owl:NamedIndividual>



    <!-- http://www.univ-tours.fr/ipato#Reconnaissance -->

    <owl:NamedIndividual rdf:about="http://www.univ-tours.fr/ipato#Reconnaissance">
        <rdf:type rdf:resource="http://www.univ-tours.fr/ipato#Forme_De_Acte"/>
        <skos:definition xml:lang="fr">Acte par lequel une personne reconnait quelque chose.</skos:definition>
        <skos:prefLabel xml:lang="fr">Reconnaissance</skos:prefLabel>
    </owl:NamedIndividual>



    <!-- http://www.univ-tours.fr/ipato#Reconnaissance_de_dette -->

    <owl:NamedIndividual rdf:about="http://www.univ-tours.fr/ipato#Reconnaissance_de_dette">
        <rdf:type rdf:resource="http://www.univ-tours.fr/ipato#Forme_De_Acte"/>
        <skos:definition xml:lang="fr">Acte par lequel une personne agissant en son nom propre ou pour le compte d&apos;un groupe de personnes atteste devoir à une autre personne une somme qui luia été prêtée ou qui reste à payer sur un marché.</skos:definition>
        <skos:prefLabel xml:lang="fr">Reconnaissance de dette</skos:prefLabel>
    </owl:NamedIndividual>



    <!-- http://www.univ-tours.fr/ipato#Renonciation -->

    <owl:NamedIndividual rdf:about="http://www.univ-tours.fr/ipato#Renonciation">
        <rdf:type rdf:resource="http://www.univ-tours.fr/ipato#Forme_De_Acte"/>
        <skos:definition xml:lang="fr">Acte par lequel une personne renonce définitivement à un droit, un bien ou une fonction, par exemple.</skos:definition>
        <skos:prefLabel xml:lang="fr">Renonciation</skos:prefLabel>
    </owl:NamedIndividual>



    <!-- http://www.univ-tours.fr/ipato#Royal_Secretary -->

    <owl:NamedIndividual rdf:about="http://www.univ-tours.fr/ipato#Royal_Secretary">
        <rdf:type rdf:resource="http://id.loc.gov/ontologies/bibframe/Role"/>
    </owl:NamedIndividual>



    <!-- http://www.univ-tours.fr/ipato#Révocation -->

    <owl:NamedIndividual rdf:about="http://www.univ-tours.fr/ipato#Révocation">
        <rdf:type rdf:resource="http://www.univ-tours.fr/ipato#Forme_De_Acte"/>
        <skos:definition xml:lang="fr">Acte par lequel une personne détentrice d&apos;une charge ou d&apos;une fonction en signifie son abandon définitif.</skos:definition>
        <skos:prefLabel xml:lang="fr">Révocation</skos:prefLabel>
    </owl:NamedIndividual>



    <!-- http://www.univ-tours.fr/ipato#Sentence -->

    <owl:NamedIndividual rdf:about="http://www.univ-tours.fr/ipato#Sentence">
        <rdf:type rdf:resource="http://www.univ-tours.fr/ipato#Forme_De_Acte"/>
        <skos:definition xml:lang="fr">Acte par lequel une instance juridique rend son jugement officiel à l&apos;encontre d&apos;une des parties mises en cause.</skos:definition>
        <skos:prefLabel xml:lang="fr">Sentence</skos:prefLabel>
    </owl:NamedIndividual>



    <!-- http://www.univ-tours.fr/ipato#Testament -->

    <owl:NamedIndividual rdf:about="http://www.univ-tours.fr/ipato#Testament">
        <rdf:type rdf:resource="http://www.univ-tours.fr/ipato#Forme_De_Acte"/>
        <skos:definition xml:lang="fr">Document officiel par lequel une personne fait part de ses dernières volontés. Un testament peu faire l&apos;objet de plusieurs versions.</skos:definition>
        <skos:prefLabel xml:lang="fr">Testament</skos:prefLabel>
    </owl:NamedIndividual>



    <!-- http://www.univ-tours.fr/ipato#Transfert -->

    <owl:NamedIndividual rdf:about="http://www.univ-tours.fr/ipato#Transfert">
        <rdf:type rdf:resource="http://www.univ-tours.fr/ipato#Forme_De_Acte"/>
        <skos:prefLabel xml:lang="fr">Transfert</skos:prefLabel>
    </owl:NamedIndividual>



    <!-- http://www.univ-tours.fr/ipato#Transfert_de_dette -->

    <owl:NamedIndividual rdf:about="http://www.univ-tours.fr/ipato#Transfert_de_dette">
        <rdf:type rdf:resource="http://www.univ-tours.fr/ipato#Forme_De_Acte"/>
        <skos:definition xml:lang="fr">Acte par lequel une personne détentrice des droits de recouvrement d&apos;une dette auprès d&apos;une autre personne ou groupe de personnes cède gratuitement ses droits à un tiers.</skos:definition>
        <skos:prefLabel xml:lang="fr">Transfert de dette</skos:prefLabel>
    </owl:NamedIndividual>



    <!-- http://www.univ-tours.fr/ipato#Transfert_de_rente -->

    <owl:NamedIndividual rdf:about="http://www.univ-tours.fr/ipato#Transfert_de_rente">
        <rdf:type rdf:resource="http://www.univ-tours.fr/ipato#Forme_De_Acte"/>
        <skos:definition xml:lang="fr">Acte par lequel une personne détentrice des droits de propriété d&apos;une rente assujettie à un bien foncier ou immobilier cède gratuitement ses droits à une autre personne.</skos:definition>
        <skos:prefLabel xml:lang="fr">Transfert de rente</skos:prefLabel>
    </owl:NamedIndividual>



    <!-- http://www.univ-tours.fr/ipato#Vente -->

    <owl:NamedIndividual rdf:about="http://www.univ-tours.fr/ipato#Vente">
        <rdf:type rdf:resource="http://www.univ-tours.fr/ipato#Forme_De_Acte"/>
        <skos:definition xml:lang="fr">Acte par lequel une personne ou un enesemble de personnes cède de façon onéreuse à une autre personne ou un autre ensemble de personne un bien foncier, mobilier ou immobilier.</skos:definition>
        <skos:prefLabel xml:lang="fr">Vente</skos:prefLabel>
    </owl:NamedIndividual>



    <!-- http://www.univ-tours.fr/ipato#centimetre -->

    <owl:NamedIndividual rdf:about="http://www.univ-tours.fr/ipato#centimetre">
        <rdf:type rdf:resource="http://erlangen-crm.org/current/E58_Measurement_Unit"/>
    </owl:NamedIndividual>



    <!-- http://www.univ-tours.fr/ipato#depth -->

    <owl:NamedIndividual rdf:about="http://www.univ-tours.fr/ipato#depth">
        <rdf:type rdf:resource="http://erlangen-crm.org/current/E55_Type"/>
    </owl:NamedIndividual>



    <!-- http://www.univ-tours.fr/ipato#height -->

    <owl:NamedIndividual rdf:about="http://www.univ-tours.fr/ipato#height">
        <rdf:type rdf:resource="http://erlangen-crm.org/current/E55_Type"/>
    </owl:NamedIndividual>



    <!-- http://www.univ-tours.fr/ipato#marriage_contract -->

    <owl:NamedIndividual rdf:about="http://www.univ-tours.fr/ipato#marriage_contract">
        <rdf:type rdf:resource="http://www.univ-tours.fr/ipato#Forme_De_Acte"/>
    </owl:NamedIndividual>



    <!-- http://www.univ-tours.fr/ipato#project_coordinator -->

    <owl:NamedIndividual rdf:about="http://www.univ-tours.fr/ipato#project_coordinator">
        <rdf:type rdf:resource="http://id.loc.gov/ontologies/bibframe/Role"/>
    </owl:NamedIndividual>



    <!-- http://www.univ-tours.fr/ipato#project_participant -->

    <owl:NamedIndividual rdf:about="http://www.univ-tours.fr/ipato#project_participant">
        <rdf:type rdf:resource="http://id.loc.gov/ontologies/bibframe/Role"/>
    </owl:NamedIndividual>



    <!-- http://www.univ-tours.fr/ipato#width -->

    <owl:NamedIndividual rdf:about="http://www.univ-tours.fr/ipato#width">
        <rdf:type rdf:resource="http://erlangen-crm.org/current/E55_Type"/>
    </owl:NamedIndividual>



    <!-- https://schema.org/editor -->

    <owl:NamedIndividual rdf:about="https://schema.org/editor">
        <rdf:type rdf:resource="http://id.loc.gov/ontologies/bibframe/Role"/>
        <rdfs:comment>Imported from schema.org</rdfs:comment>
        <skos:prefLabel xml:lang="en">editor</skos:prefLabel>
    </owl:NamedIndividual>



    <!--
    ///////////////////////////////////////////////////////////////////////////////////////
    //
    // General axioms
    //
    ///////////////////////////////////////////////////////////////////////////////////////
     -->

    <rdf:Description>
        <rdf:type rdf:resource="http://www.w3.org/2002/07/owl#AllDisjointClasses"/>
        <owl:members rdf:parseType="Collection">
            <rdf:Description rdf:about="http://www.univ-tours.fr/ipato#Research_Area"/>
            <rdf:Description rdf:about="http://www.w3.org/ns/dcat#Catalog"/>
            <rdf:Description rdf:about="http://www.w3.org/ns/dcat#Dataset"/>
        </owl:members>
    </rdf:Description>
</rdf:RDF>



<!-- Generated by the OWL API (version 4.5.9.2019-02-01T07:24:44Z) https://github.com/owlcs/owlapi -->
